src/definitions3.lean
@@ -96,122 +96,6 @@ inductive vc.uses_var (x: var) : vc → Prop
 | univ {y: var} {P: vc}                 : vc.uses_var P → vc.uses_var (vc.univ y P)
 | quantified {P: vc}                    : vc.uses_var (vc.univ x P)
 
--- verification conditions without quantifier instantiation algorithm
-
-notation `⦃` P `⦄`: 100 := ∀ (σ: env), closed_subst σ P → σ ⊨ P.to_vc
-
-reserve infix `⊩`:10
-
--- verification of expressions
-
-inductive exp.dvcgen : prop → exp → propctx → Prop
-notation P `⊩` e `:` Q : 10 := exp.dvcgen P e Q
-
-| tru {P: prop} {x: var} {e: exp} {Q: propctx}:
-    x ∉ FV P →
-    (P ⋀ x ≡ value.true ⊩ e : Q) →
-    (P ⊩ lett x = true in e : propctx.exis x (x ≡ value.true ⋀ Q))
-
-| fals {P: prop} {x: var} {e: exp} {Q: propctx}:
-    x ∉ FV P →
-    (P ⋀ x ≡ value.false ⊩ e : Q) →
-    (P ⊩ letf x = false in e : propctx.exis x (x ≡ value.false ⋀ Q))
-
-| num {P: prop} {x: var} {n: ℕ} {e: exp} {Q: propctx}:
-    x ∉ FV P →
-    (P ⋀ x ≡ value.num n ⊩ e : Q) →
-    (P ⊩ letn x = n in e : propctx.exis x (x ≡ value.num n ⋀ Q))
-
-| func {P: prop} {f x: var} {R S: spec} {e₁ e₂: exp} {Q₁ Q₂: propctx}:
-    f ∉ FV P →
-    x ∉ FV P →
-    f ≠ x →
-    x ∈ FV R.to_prop.to_vc →
-    FV R.to_prop ⊆ FV P ∪ { f, x } →
-    FV S.to_prop ⊆ FV P ∪ { f, x } →
-    (P ⋀ spec.func f x R S ⋀ R ⊩ e₁ : Q₁) →
-    (P ⋀ prop.func f x R (Q₁ (term.app f x) ⋀ S) ⊩ e₂ : Q₂) →
-    ⦃ prop.implies (P ⋀ spec.func f x R S ⋀ R ⋀ Q₁ (term.app f x)) S ⦄ →
-    (P ⊩ letf f[x] req R ens S {e₁} in e₂ : propctx.exis f (prop.func f x R (Q₁ (term.app f x) ⋀ S) ⋀ Q₂))
-
-| unop {P: prop} {op: unop} {e: exp} {x y: var} {Q: propctx}:
-    x ∈ FV P →
-    y ∉ FV P →
-    (P ⋀ y ≡ term.unop op x ⊩ e : Q) →
-    ⦃ prop.implies P (prop.pre₁ op x) ⦄ →
-    (P ⊩ letop y = op [x] in e : propctx.exis y (y ≡ term.unop op x ⋀ Q))
-
-| binop {P: prop} {op: binop} {e: exp} {x y z: var} {Q: propctx}:
-    x ∈ FV P →
-    y ∈ FV P →
-    z ∉ FV P →
-    (P ⋀ z ≡ term.binop op x y ⊩ e : Q) →
-    ⦃ prop.implies P (prop.pre₂ op x y) ⦄ →
-    (P ⊩ letop2 z = op [x, y] in e : propctx.exis z (z ≡ term.binop op x y ⋀ Q))
-
-| app {P: prop} {e: exp} {y f x: var} {Q: propctx}:
-    f ∈ FV P →
-    x ∈ FV P →
-    y ∉ FV P →
-    (P ⋀ prop.call f x ⋀ prop.post f x ⋀ y ≡ term.app f x ⊩ e : Q) →
-    ⦃ prop.implies (P ⋀ prop.call f x) (term.unop unop.isFunc f ⋀ prop.pre f x) ⦄ →
-    (P ⊩ letapp y = f [x] in e : propctx.exis y (prop.call f x ⋀ prop.post f x ⋀ y ≡ term.app f x ⋀ Q))
-
-| ite {P: prop} {e₁ e₂: exp} {x: var} {Q₁ Q₂: propctx}:
-    x ∈ FV P →
-    (P ⋀ x ⊩ e₁ : Q₁) →
-    (P ⋀ prop.not x ⊩ e₂ : Q₂) →
-    ⦃ prop.implies P (term.unop unop.isBool x) ⦄ →
-    (P ⊩ exp.ite x e₁ e₂ : propctx.implies x Q₁ ⋀ propctx.implies (prop.not x) Q₂)
-
-| return {P: prop} {x: var}:
-    x ∈ FV P →
-    (P ⊩ exp.return x : x ≣ •)
-
-notation P `⊩` e `:` Q : 10 := exp.dvcgen P e Q
-
--- verification of environments/translation into logic
-
-inductive env.dvcgen : env → prop → Prop
-notation `⊩` σ `:` Q : 10 := env.dvcgen σ Q
-
-| empty:
-    ⊩ env.empty : value.true
-
-| tru {σ: env} {x: var} {Q: prop}:
-    x ∉ σ →
-    (⊩ σ : Q) →
-    (⊩ (σ[x ↦ value.true]) : Q ⋀ x ≡ value.true)
-
-| fls {σ: env} {x: var} {Q: prop}:
-    x ∉ σ →
-    (⊩ σ : Q) →
-    (⊩ (σ[x ↦ value.false]) : Q ⋀ x ≡ value.false)
-
-| num {n: ℤ} {σ: env} {x: var} {Q: prop}:
-    x ∉ σ →
-    (⊩ σ : Q) →
-    (⊩ (σ[x ↦ value.num n]) : Q ⋀ x ≡ value.num n)
-
-| func {σ₁ σ₂: env} {f g x: var} {R S: spec} {e: exp} {Q₁ Q₂: prop} {Q₃: propctx}:
-    f ∉ σ₁ →
-    g ∉ σ₂ →
-    x ∉ σ₂ →
-    g ≠ x →
-    (⊩ σ₁ : Q₁) →
-    (⊩ σ₂ : Q₂) →
-    x ∈ FV R.to_prop.to_vc →
-    FV R.to_prop ⊆ FV Q₂ ∪ { g, x } →
-    FV S.to_prop ⊆ FV Q₂ ∪ { g, x } →
-    (Q₂ ⋀ spec.func g x R S ⋀ R ⊩ e : Q₃) →
-    ⦃ prop.implies (Q₂ ⋀ spec.func g x R S ⋀ R ⋀ Q₃ (term.app g x)) S ⦄ →
-    (⊩ (σ₁[f ↦ value.func g x R S e σ₂]) :
-      (Q₁
-       ⋀ f ≡ value.func g x R S e σ₂
-       ⋀ prop.subst_env (σ₂[g↦value.func g x R S e σ₂]) (prop.func g x R (Q₃ (term.app g x) ⋀ S))))
-
-notation `⊩` σ `:` Q : 10 := env.dvcgen σ Q
-
 -- runtime verification of stacks
 
 inductive stack.dvcgen : stack → propctx → Prop
@@ -220,7 +104,7 @@ notation `⊩ₛ` s `:` Q : 10 := stack.dvcgen s Q
 | top {R: spec} {P: prop} {σ: env} {e: exp} {Q: propctx}:
     (⊩ σ : P) →
     FV R.to_prop ⊆ FV P →
-    (σ ⊨ R.to_prop.instantiated_n) →
+    (σ ⊨ R.to_prop.to_vc) →
     (R ⋀ P ⊩ e : Q) →
     (⊩ₛ (R, σ, e) : P ⋀ Q)
 
@@ -235,13 +119,13 @@ notation `⊩ₛ` s `:` Q : 10 := stack.dvcgen s Q
     (σ₁ ⊨ R₁.to_prop.to_vc) →
     (σ₁ g = value.func f fx R₂ S₂ e₂ σ₂) →
     (σ₁ x = v) →
-    (R₁ ⋀ P₁ ⋀ prop.call g x ⋀ prop.post g x ⋀ y ≡ term.app g x ⊩ e₁ : Q₁) →
+    (R₁ ⋀ P₁ ⋀ prop.call x ⋀ prop.post g x ⋀ y ≡ term.app g x ⊩ e₁ : Q₁) →
     (P₂ ⋀ spec.func f fx R₂ S₂ ⋀ R₂ ⊩ e₂ : Q₂) →
     (∀σ' t, (σ' ⊨ (Q₂' t).to_vc) → σ' ⊨ (P₃ ⋀ (Q₂ t)).to_vc) →
     (∀v: value, FV (P₃ ⋀ (Q₂ v)) ⊆ FV (Q₂' v)) →
-    ⦃ prop.implies (R₁ ⋀ P₁ ⋀ prop.call g x) (term.unop unop.isFunc g ⋀ prop.pre g x) ⦄ →
+    ⦃ prop.implies (R₁ ⋀ P₁ ⋀ prop.call x) (term.unop unop.isFunc g ⋀ prop.pre g x) ⦄ →
     ((R₂, σ₂[f↦value.func f fx R₂ S₂ e₂ σ₂][fx↦v], e₂) ⟶* s) →
     (⊩ₛ (s · [R₁, σ₁, letapp y = g[x] in e₁]) : P₁ ⋀
-          propctx.exis y (prop.call g x ⋀ prop.post g x ⋀ y ≡ term.app g x ⋀ Q₁))
+          propctx.exis y (prop.call x ⋀ prop.post g x ⋀ y ≡ term.app g x ⋀ Q₁))
 
 notation `⊩ₛ` s `:` Q : 10 := stack.dvcgen s Q
