src/progress.lean
@@ -1,52 +1,51 @@
-/-
-import .definitions2
+import .definitions3 .logic
 
 @[reducible]
 def is_value(s: stack): Prop :=
-  ∃(R: spec) (H: history) (σ: env) (x: var) (v: value), s = (R, H, σ, exp.return x) ∧ (σ x = v)
+  ∃(R: spec) (σ: env) (x: var) (v: value), s = (R, σ, exp.return x) ∧ (σ x = v)
 
-lemma exp.progress {R: spec} {H: history} {P: prop} {Q: propctx} {e: exp} {σ: env}:
-      (⊢ σ: P) → (FV R.to_prop ⊆ FV P) → (σ ⊨ R.to_prop.instantiated_n) → (R ⋀ H ⋀ P ⊢ e: Q) → 
-      is_value (R, H, σ, e) ∨ ∃s', (R, H, σ, e) ⟶ s' :=
-  assume env_verified: (⊢ σ : P),
+lemma exp.progress {R: spec} {P: prop} {Q: propctx} {e: exp} {σ: env}:
+      (⊩ σ: P) → (FV R.to_prop ⊆ FV P) → (σ ⊨ R.to_prop.to_vc) → (R ⋀ P ⊩ e: Q) → 
+      is_value (R, σ, e) ∨ ∃s', (R, σ, e) ⟶ s' :=
+  assume env_verified: (⊩ σ : P),
   assume fv_R: FV R.to_prop ⊆ FV P,
-  assume R_valid: (σ ⊨ R.to_prop.instantiated_n),
-  assume e_verified: (R ⋀ H ⋀ P ⊢ e : Q),
+  assume R_valid: (σ ⊨ R.to_prop.to_vc),
+  assume e_verified: (R ⋀ P ⊩ e : Q),
   have R_closed: closed_subst σ R.to_prop, from (
     assume z: var,
     assume : z ∈ FV R.to_prop,
     have z ∈ FV P, from set.mem_of_subset_of_mem fv_R this,
     show z ∈ σ.dom, from (free_iff_contains env_verified).symm ▸ this
   ),
-  show is_value (R, H, σ, e) ∨ ∃s', (R, H, σ, e) ⟶ s', by begin
+  show is_value (R, σ, e) ∨ ∃s', (R, σ, e) ⟶ s', by begin
     cases e_verified,
-    case exp.vcgen.tru x e' { from
-      let s: stack := (R, H, σ, lett x = true in e') in
-      have s ⟶ (R, H, σ[x↦value.true], e'), from step.tru,
-      have ∃s', s ⟶ s', from exists.intro (R, H, σ[x↦value.true], e') this,
+    case exp.dvcgen.tru x e' { from
+      let s: stack := (R, σ, lett x = true in e') in
+      have s ⟶ (R, σ[x↦value.true], e'), from step.tru,
+      have ∃s', s ⟶ s', from exists.intro (R, σ[x↦value.true], e') this,
       show is_value s ∨ ∃s', s ⟶ s', from or.inr this
     },
-    case exp.vcgen.fals x e' { from
-      let s: stack := (R, H, σ, letf x = false in e') in
-      have s ⟶ (R, H, σ[x↦value.false], e'), from step.fals,
-      have ∃s', s ⟶ s', from exists.intro (R, H, σ[x↦value.false], e') this,
+    case exp.dvcgen.fals x e' { from
+      let s: stack := (R, σ, letf x = false in e') in
+      have s ⟶ (R, σ[x↦value.false], e'), from step.fals,
+      have ∃s', s ⟶ s', from exists.intro (R, σ[x↦value.false], e') this,
       show is_value s ∨ ∃s', s ⟶ s', from or.inr this
     },
-    case exp.vcgen.num x n e' { from
-      let s: stack := (R, H, σ, letn x = n in e') in
-      have s ⟶ (R, H, σ[x↦value.num n], e'), from step.num,
-      have ∃s', s ⟶ s', from exists.intro (R, H, σ[x↦value.num n], e') this,
+    case exp.dvcgen.num x n e' { from
+      let s: stack := (R, σ, letn x = n in e') in
+      have s ⟶ (R, σ[x↦value.num n], e'), from step.num,
+      have ∃s', s ⟶ s', from exists.intro (R, σ[x↦value.num n], e') this,
       show is_value s ∨ ∃s', s ⟶ s', from or.inr this
     },
-    case exp.vcgen.func f x R' S' e₁ e₂ { from
-      let s: stack := (R, H, σ, letf f[x] req R' ens S' {e₁} in e₂) in
-      have s ⟶ (R, H, σ[f↦value.func f x R' S' e₁ H σ], e₂), from step.closure,
-      have ∃s', s ⟶ s', from exists.intro (R, H, σ[f↦value.func f x R' S' e₁ H σ], e₂) this,
+    case exp.dvcgen.func f x R' S' e₁ e₂ { from
+      let s: stack := (R, σ, letf f[x] req R' ens S' {e₁} in e₂) in
+      have s ⟶ (R, σ[f↦value.func f x R' S' e₁ σ], e₂), from step.closure,
+      have ∃s', s ⟶ s', from exists.intro (R, σ[f↦value.func f x R' S' e₁ σ], e₂) this,
       show is_value s ∨ ∃s', s ⟶ s', from or.inr this
     },
-    case exp.vcgen.unop op x y e' Q' x_free_in_P _ e'_verified vc_valid { from
-      let s: stack := (R, H, σ, letop y = op[x] in e') in
-      let ⟨v, env_has_x⟩ := (val_of_free_in_hist_env env_verified fv_R x_free_in_P) in
+    case exp.dvcgen.unop op x y e' Q' x_free_in_P _ e'_verified vc_valid { from
+      let s: stack := (R, σ, letop y = op[x] in e') in
+      let ⟨v, env_has_x⟩ := (val_of_free_in_pre_env env_verified fv_R x_free_in_P) in
       have closed_subst σ (prop.pre₁ op x), from (
         assume z: var,
         assume : z ∈ FV (prop.pre₁ op x),
@@ -54,9 +53,8 @@ lemma exp.progress {R: spec} {H: history} {P: prop} {Q: propctx} {e: exp} {σ: e
         have z = x, from free_in_term.var.inv this,
         show z ∈ σ, from this.symm ▸ env.contains_apply_equiv.right.mp (exists.intro v env_has_x)
       ),
-      have σ ⊨ (prop.pre₁ op x).instantiated_p, from consequent_of_H_P env_verified R_closed R_valid this vc_valid,
-      have h1: σ ⊨ (prop.pre₁ op x).erased_p, from valid_env.erased_p_of_instantiated_p this,
-      have (prop.pre₁ op x).erased_p = vc.pre₁ op x, by unfold prop.erased_p,
+      have h1: σ ⊨ (prop.pre₁ op x).to_vc, from consequent_of_pre_P env_verified R_closed R_valid this vc_valid,
+      have (prop.pre₁ op x).to_vc = vc.pre₁ op x, by unfold prop.to_vc,
       have h2: ⊨ vc.subst_env σ (vc.pre₁ op x), from this ▸ h1,
       have vc.subst_env σ (vc.pre₁ op x) = vc.pre₁ op (term.subst_env σ x), from vc.subst_env.pre₁,
       have ⊨ vc.pre₁ op (term.subst_env σ x), from this ▸ h2,
@@ -65,14 +63,14 @@ lemma exp.progress {R: spec} {H: history} {P: prop} {Q: propctx} {e: exp} {σ: e
       have option.is_some (unop.apply op v), from valid.pre₁.mpr this,
       have (∃v', unop.apply op v = some v'), from option.is_some_iff_exists.mp this,
       let ⟨v', op_v_is_v'⟩ := this in
-      have s ⟶ (R, H, σ[y↦v'], e'), from step.unop env_has_x op_v_is_v',
-      have ∃s', s ⟶ s', from exists.intro (R, H, σ[y↦v'], e') this,
+      have s ⟶ (R, σ[y↦v'], e'), from step.unop env_has_x op_v_is_v',
+      have ∃s', s ⟶ s', from exists.intro (R, σ[y↦v'], e') this,
       show is_value s ∨ ∃s', s ⟶ s', from or.inr this
     },
-    case exp.vcgen.binop op x y z e' Q' x_free_in_P y_free_in_P _ e'_verified vc_valid { from
-      let s: stack := (R, H, σ, letop2 z = op[x,y] in e') in
-      let ⟨vx, env_has_x⟩ := (val_of_free_in_hist_env env_verified fv_R x_free_in_P) in
-      let ⟨vy, env_has_y⟩ := (val_of_free_in_hist_env env_verified fv_R y_free_in_P) in
+    case exp.dvcgen.binop op x y z e' Q' x_free_in_P y_free_in_P _ e'_verified vc_valid { from
+      let s: stack := (R, σ, letop2 z = op[x,y] in e') in
+      let ⟨vx, env_has_x⟩ := (val_of_free_in_pre_env env_verified fv_R x_free_in_P) in
+      let ⟨vy, env_has_y⟩ := (val_of_free_in_pre_env env_verified fv_R y_free_in_P) in
       have closed_subst σ (prop.pre₂ op x y), from (
         assume z: var,
         assume : z ∈ FV (prop.pre₂ op x y),
@@ -86,9 +84,8 @@ lemma exp.progress {R: spec} {H: history} {P: prop} {Q: propctx} {e: exp} {σ: e
           show z ∈ σ, from this.symm ▸ env.contains_apply_equiv.right.mp (exists.intro vy env_has_y)
         )
       ),
-      have σ ⊨ (prop.pre₂ op x y).instantiated_p, from consequent_of_H_P env_verified R_closed R_valid this vc_valid,
-      have h1: σ ⊨ (prop.pre₂ op x y).erased_p, from valid_env.erased_p_of_instantiated_p this,
-      have (prop.pre₂ op x y).erased_p = vc.pre₂ op x y, by unfold prop.erased_p,
+      have h1: σ ⊨ (prop.pre₂ op x y).to_vc, from consequent_of_pre_P env_verified R_closed R_valid this vc_valid,
+      have (prop.pre₂ op x y).to_vc = vc.pre₂ op x y, by unfold prop.to_vc,
       have h2: ⊨ vc.subst_env σ (vc.pre₂ op x y), from this ▸ h1,
       have vc.subst_env σ (vc.pre₂ op x y) = vc.pre₂ op (term.subst_env σ x) (term.subst_env σ y),
       from vc.subst_env.pre₂,
@@ -100,15 +97,15 @@ lemma exp.progress {R: spec} {H: history} {P: prop} {Q: propctx} {e: exp} {σ: e
       have option.is_some (binop.apply op vx vy), from valid.pre₂.mpr this,
       have (∃v', binop.apply op vx vy = some v'), from option.is_some_iff_exists.mp this,
       let ⟨v', op_v_is_v'⟩ := this in
-      have s ⟶ (R, H, σ[z↦v'], e'), from step.binop env_has_x env_has_y op_v_is_v',
-      have ∃s', s ⟶ s', from exists.intro (R, H, σ[z↦v'], e') this,
+      have s ⟶ (R, σ[z↦v'], e'), from step.binop env_has_x env_has_y op_v_is_v',
+      have ∃s', s ⟶ s', from exists.intro (R, σ[z↦v'], e') this,
       show is_value s ∨ ∃s', s ⟶ s', from or.inr this
     },
-    case exp.vcgen.app y f x e' Q' f_free_in_P x_free_in_P _ e'_verified vc_valid { from
-      let s: stack := (R, H, σ, letapp y = f [x] in e') in
-      let ⟨vf, env_f_is_vf⟩ := (val_of_free_in_hist_env env_verified fv_R f_free_in_P) in
+    case exp.dvcgen.app y f x e' Q' f_free_in_P x_free_in_P _ e'_verified vc_valid { from
+      let s: stack := (R, σ, letapp y = f [x] in e') in
+      let ⟨vf, env_f_is_vf⟩ := (val_of_free_in_pre_env env_verified fv_R f_free_in_P) in
       have env_has_f: f ∈ σ, from env.contains_apply_equiv.right.mp (exists.intro vf env_f_is_vf),
-      let ⟨vx, env_x_is_vx⟩ := (val_of_free_in_hist_env env_verified fv_R x_free_in_P) in
+      let ⟨vx, env_x_is_vx⟩ := (val_of_free_in_pre_env env_verified fv_R x_free_in_P) in
       have env_has_x: x ∈ σ, from env.contains_apply_equiv.right.mp (exists.intro vx env_x_is_vx),
       have closed_subst σ (↑(term.unop unop.isFunc f) ⋀ prop.pre f x), from (
         assume z: var,
@@ -132,22 +129,22 @@ lemma exp.progress {R: spec} {H: history} {P: prop} {Q: propctx} {e: exp} {σ: e
           )
         )
       ),
-      have σ ⊨ (↑(term.unop unop.isFunc f) ⋀ prop.pre f x).instantiated_p,
-      from consequent_of_H_P_call env_verified R_closed R_valid vc_valid env_has_f env_has_x this,
-      have h3: σ ⊨ (↑(term.unop unop.isFunc f) ⋀ prop.pre f x).erased_p,
-      from valid_env.erased_p_of_instantiated_p this,
-      have (prop.and (prop.term (term.unop unop.isFunc f)) (prop.pre f x)).erased_p
-         = ((prop.term (term.unop unop.isFunc f)).erased_p ⋀ (prop.pre f x).erased_p), by unfold prop.erased_p,
-      have σ ⊨ ((prop.term (term.unop unop.isFunc f)).erased_p ⋀ (prop.pre f x).erased_p), from this ▸ h3,
-      have h4: ⊨ vc.subst_env σ ((prop.term (term.unop unop.isFunc f)).erased_p ⋀ (prop.pre f x).erased_p), from this,
-      have vc.subst_env σ ((prop.term (term.unop unop.isFunc f)).erased_p ⋀ (prop.pre f x).erased_p)
-         = (vc.subst_env σ ((prop.term (term.unop unop.isFunc f)).erased_p) ⋀ vc.subst_env σ ((prop.pre f x).erased_p)),
+      have h1: σ ⊨ (↑(term.unop unop.isFunc f) ⋀ prop.pre f x).to_vc,
+      from consequent_of_pre_P_call env_verified R_closed R_valid env_has_x this vc_valid,
+      have (prop.and (prop.term (term.unop unop.isFunc f)) (prop.pre f x)).to_vc
+         = ((prop.term (term.unop unop.isFunc f)).to_vc ⋀ (prop.pre f x).to_vc),
+      by unfold prop.to_vc,
+      have σ ⊨ ((prop.term (term.unop unop.isFunc f)).to_vc ⋀ (prop.pre f x).to_vc), from this ▸ h1,
+      have h2: ⊨ vc.subst_env σ ((prop.term (term.unop unop.isFunc f)).to_vc ⋀ (prop.pre f x).to_vc), from this,
+      have vc.subst_env σ ((prop.term (term.unop unop.isFunc f)).to_vc ⋀ (prop.pre f x).to_vc)
+         = (vc.subst_env σ ((prop.term (term.unop unop.isFunc f)).to_vc) ⋀ vc.subst_env σ ((prop.pre f x).to_vc)),
       from vc.subst_env.and,
-      have ⊨ (vc.subst_env σ ((prop.term (term.unop unop.isFunc f)).erased_p) ⋀ vc.subst_env σ ((prop.pre f x).erased_p)),
-      from this ▸ h4,
-      have h5: σ ⊨ (prop.term (term.unop unop.isFunc f)).erased_p, from (valid.and.mpr this).left,
-      have (prop.term (term.unop unop.isFunc f)).erased_p = vc.term (term.unop unop.isFunc f),
-      by unfold prop.erased_p,
+      have ⊨ (vc.subst_env σ ((prop.term (term.unop unop.isFunc f)).to_vc) ⋀
+              vc.subst_env σ ((prop.pre f x).to_vc)),
+      from this ▸ h2,
+      have h5: σ ⊨ (prop.term (term.unop unop.isFunc f)).to_vc, from (valid.and.mpr this).left,
+      have (prop.term (term.unop unop.isFunc f)).to_vc = vc.term (term.unop unop.isFunc f),
+      by unfold prop.to_vc,
       have h6: σ ⊨ vc.term (term.unop unop.isFunc f), from this ▸ h5,
       have vc.subst_env σ (vc.term (term.unop unop.isFunc f)) = vc.term (term.subst_env σ (term.unop unop.isFunc f)),
       from vc.subst_env.term,
@@ -159,19 +156,19 @@ lemma exp.progress {R: spec} {H: history} {P: prop} {Q: propctx} {e: exp} {σ: e
       have ⊨ term.unop unop.isFunc vf, from this ▸ h8,
       have ⊨ (value.true ≡ term.unop unop.isFunc vf), from valid.eq.true.mp this,
       have unop.apply unop.isFunc vf = some value.true, from valid.unop.mpr this,
-      have ∃(g gx: var) (gR gS: spec) (ge: exp) (gH: history) (gσ: env), vf = value.func g gx gR gS ge gH gσ,
+      have ∃(g gx: var) (gR gS: spec) (ge: exp) (gσ: env), vf = value.func g gx gR gS ge gσ,
       from unop.isFunc.inv this,
-      let ⟨g, gx, gR, gS, ge, gH, gσ, vf_is_g⟩ := this in
-      have some_vf_is_g: some vf = ↑(value.func g gx gR gS ge gH gσ), from some.inj.inv vf_is_g,
-      have σ f = value.func g gx gR gS ge gH gσ, from eq.trans env_f_is_vf some_vf_is_g,
-      let s': stack := (gR, gH, gσ[g↦value.func g gx gR gS ge gH gσ][gx↦vx], ge) · [R, H, σ, letapp y = f[x] in e'] in
+      let ⟨g, gx, gR, gS, ge, gσ, vf_is_g⟩ := this in
+      have some_vf_is_g: some vf = ↑(value.func g gx gR gS ge gσ), from some.inj.inv vf_is_g,
+      have σ f = value.func g gx gR gS ge gσ, from eq.trans env_f_is_vf some_vf_is_g,
+      let s': stack := (gR, gσ[g↦value.func g gx gR gS ge gσ][gx↦vx], ge) · [R, σ, letapp y = f[x] in e'] in
       have s ⟶ s', from step.app this env_x_is_vx,
       have ∃s', s ⟶ s', from exists.intro s' this,
       show is_value s ∨ ∃s', s ⟶ s', from or.inr this
     },
-    case exp.vcgen.ite x e₂ e₁ Q₁ Q₂ x_free_in_P _ _ vc_valid { from
-      let s: stack := (R, H, σ, exp.ite x e₁ e₂) in
-      let ⟨v, env_has_x⟩ := (val_of_free_in_hist_env env_verified fv_R x_free_in_P) in
+    case exp.dvcgen.ite x e₂ e₁ Q₁ Q₂ x_free_in_P _ _ vc_valid { from
+      let s: stack := (R, σ, exp.ite x e₁ e₂) in
+      let ⟨v, env_has_x⟩ := (val_of_free_in_pre_env env_verified fv_R x_free_in_P) in
       have closed_subst σ (prop.term (term.unop unop.isBool x)), from (
         assume z: var,
         assume : z ∈ FV (prop.term (term.unop unop.isBool x)),
@@ -180,12 +177,10 @@ lemma exp.progress {R: spec} {H: history} {P: prop} {Q: propctx} {e: exp} {σ: e
         have z = x, from free_in_term.var.inv this,
         show z ∈ σ, from this.symm ▸ env.contains_apply_equiv.right.mp (exists.intro v env_has_x)
       ),
-      have σ ⊨ (prop.term (term.unop unop.isBool x)).instantiated_p,
-      from consequent_of_H_P env_verified R_closed R_valid this vc_valid,
-      have h1: σ ⊨ (prop.term (term.unop unop.isBool x)).erased_p,
-      from valid_env.erased_p_of_instantiated_p this,
-      have (prop.term (term.unop unop.isBool x)).erased_p = vc.term (term.unop unop.isBool x),
-      by unfold prop.erased_p,
+      have h1: σ ⊨ (prop.term (term.unop unop.isBool x)).to_vc,
+      from consequent_of_pre_P env_verified R_closed R_valid this vc_valid,
+      have (prop.term (term.unop unop.isBool x)).to_vc = vc.term (term.unop unop.isBool x),
+      by unfold prop.to_vc,
       have h2: σ ⊨ vc.term (term.unop unop.isBool x), from this ▸ h1,
       have vc.subst_env σ (vc.term (term.unop unop.isBool x)) = vc.term (term.subst_env σ (term.unop unop.isBool x)),
       from vc.subst_env.term,
@@ -202,65 +197,63 @@ lemma exp.progress {R: spec} {H: history} {P: prop} {Q: propctx} {e: exp} {σ: e
         assume : v = value.true,
         have some v = some value.true, from some.inj.inv this,
         have σ x = value.true, from eq.trans env_has_x this,
-        have s ⟶ (R, H, σ, e₁), from step.ite_true this,
-        have ∃s', s ⟶ s', from exists.intro (R, H, σ, e₁) this,
+        have s ⟶ (R, σ, e₁), from step.ite_true this,
+        have ∃s', s ⟶ s', from exists.intro (R, σ, e₁) this,
         show is_value s ∨ ∃s', s ⟶ s', from or.inr this
       ) (
         assume : v = value.false,
         have some v = some value.false, from some.inj.inv this,
         have σ x = value.false, from eq.trans env_has_x this,
-        have s ⟶ (R, H, σ, e₂), from step.ite_false this,
-        have ∃s', s ⟶ s', from exists.intro (R, H, σ, e₂) this,
+        have s ⟶ (R, σ, e₂), from step.ite_false this,
+        have ∃s', s ⟶ s', from exists.intro (R, σ, e₂) this,
         show is_value s ∨ ∃s', s ⟶ s', from or.inr this
       )
     },
-    case exp.vcgen.return x x_free_in_P { from
-      let s: stack := (R, H, σ, exp.return x) in
-      have s_is_return: s = (R, H, σ, exp.return x), from rfl,
-      let ⟨v, env_has_x⟩ := (val_of_free_in_hist_env env_verified fv_R x_free_in_P) in
+    case exp.dvcgen.return x x_free_in_P { from
+      let s: stack := (R, σ, exp.return x) in
+      have s_is_return: s = (R, σ, exp.return x), from rfl,
+      let ⟨v, env_has_x⟩ := (val_of_free_in_pre_env env_verified fv_R x_free_in_P) in
       have is_value_s: is_value s
-        = (∃(R': spec) (H': history) (σ': env) (x': var) (v: value), s = (R', H', σ', exp.return x') ∧ (σ' x' = v)),
+        = (∃(R': spec) (σ': env) (x': var) (v: value), s = (R', σ', exp.return x') ∧ (σ' x' = v)),
       by unfold is_value,
-      have (∃(R': spec) (H': history) (σ': env) (x': var) (v: value), s = (R', H', σ', exp.return x') ∧ (σ' x' = v)),
-      from exists.intro R (exists.intro H (exists.intro σ (exists.intro x (exists.intro v ⟨s_is_return, env_has_x⟩)))),
+      have (∃(R': spec) (σ': env) (x': var) (v: value), s = (R', σ', exp.return x') ∧ (σ' x' = v)),
+      from exists.intro R (exists.intro σ (exists.intro x (exists.intro v ⟨s_is_return, env_has_x⟩))),
       have is_value s, from is_value_s ▸ this,
       show is_value s ∨ ∃s', s ⟶ s', from or.inl this
     }
   end
 
-theorem progress {s: stack} {Q: propctx}: (⊢ₛ s : Q) → is_value s ∨ ∃s', s ⟶ s'
+theorem progress {s: stack} {Q: propctx}: (⊩ₛ s : Q) → is_value s ∨ ∃s', s ⟶ s'
 :=
-  assume s_verified: ⊢ₛ s : Q,
+  assume s_verified: ⊩ₛ s : Q,
   begin
     induction s_verified,
-    case stack.vcgen.top σ e Q R H P env_verified fv_R R_valid e_verified { from
-      show is_value (R, H, σ, e) ∨ ∃s', (R, H, σ, e) ⟶ s', from exp.progress env_verified fv_R R_valid e_verified
+    case stack.dvcgen.top σ e R P Q env_verified fv_R R_valid e_verified { from
+      show is_value (R, σ, e) ∨ ∃s', (R, σ, e) ⟶ s', from exp.progress env_verified fv_R R_valid e_verified
     },
-    case stack.vcgen.cons H' H P P' P'' s' σ σ' f g x y fx R R' S' e₁ e₂ vₓ Q Q' Q''
+    case stack.dvcgen.cons P P' P'' s' σ σ' f g x y fx R R' S' e₁ e₂ vₓ Q Q' Q''
                           s'_verified y_not_in_σ σ_verified σ'_verified σ''_verified fv_R R_valid g_is_func
-                          x_is_v e₁_verified cont Q''_dom pre_vc steps ih { from
-      let s := (s' · [R, H', σ, letapp y = g[x] in e₁]) in
-      have s_cons: s = (s' · [R, H', σ, letapp y = g[x] in e₁]), from rfl,
+                          x_is_v e₁_verified cont Q''_dom Q''_fv pre_vc steps ih { from
+      let s := (s' · [R, σ, letapp y = g[x] in e₁]) in
+      have s_cons: s = (s' · [R, σ, letapp y = g[x] in e₁]), from rfl,
       or.elim ih
       ( -- step return
         assume s'_is_value: is_value s',
-        let ⟨R₂, H₂, σ₂, z, v, ⟨s'_return, env2_has_z⟩⟩ := s'_is_value in
-        have s_return_cons: s = ((R₂, H₂, σ₂, exp.return z) · [R, H', σ, letapp y = g[x] in e₁]),
+        let ⟨R₂, σ₂, z, v, ⟨s'_return, env2_has_z⟩⟩ := s'_is_value in
+        have s_return_cons: s = ((R₂, σ₂, exp.return z) · [R, σ, letapp y = g[x] in e₁]),
         from s'_return ▸ s_cons,
-        have s ⟶ (R, H' · call f fx R' S' e₂ H σ' vₓ, σ[y↦v], e₁),
+        have s ⟶ (R, σ[y↦v], e₁),
         from s_return_cons.symm ▸ (step.return env2_has_z g_is_func x_is_v),
         have ∃s', s ⟶ s',
-        from exists.intro (R, H' · call f fx R' S' e₂ H σ' vₓ, σ[y↦v], e₁) this,
+        from exists.intro (R, σ[y↦v], e₁) this,
         show is_value s ∨ ∃s', s ⟶ s', from or.inr this
       )
       ( -- step ctx
         assume s'_can_step: ∃s'', s' ⟶ s'',
         let ⟨s'', s'_steps⟩ := s'_can_step in
-        have s ⟶ (s'' · [R, H', σ, letapp y = g[x] in e₁]), from step.ctx s'_steps,
-        have ∃s', s ⟶ s', from exists.intro (s'' · [R, H', σ, letapp y = g[x] in e₁]) this,
+        have s ⟶ (s'' · [R, σ, letapp y = g[x] in e₁]), from step.ctx s'_steps,
+        have ∃s', s ⟶ s', from exists.intro (s'' · [R, σ, letapp y = g[x] in e₁]) this,
         show is_value s ∨ ∃s', s ⟶ s', from or.inr this
       )
     }
   end
-
--/
