src/logic.lean
@@ -296,7 +296,6 @@ lemma valid.alpha_equiv {x y: var} {P: vc}: (⊨ P) → ⊨ vc.substt x y P :=
   end
 
 /-
-
 lemma valid_env.subst_of_eq_instantiated_p {σ: env} {x: var} {v: value}:
       (σ ⊨ prop.instantiated_p (x ≡ v)) → (σ x = v) :=
   assume h0: σ ⊨ prop.instantiated_p (x ≡ v),
@@ -328,85 +327,76 @@ lemma valid_env.subst_of_eq_instantiated_n {σ: env} {x: var} {v: value}:
   by unfold prop.erased_n,
   have σ ⊨ vc.term (x ≡ v), from this.symm ▸ h1,
   show σ x = v, from valid_env.subst_of_eq this
+-/
 
-lemma history_valid {H: history}: ⟪calls_to_prop H⟫ :=
-  assume σ: env,
+lemma valid.to_vc_and {P Q: prop}: (⊨ P.to_vc) → (⊨ Q.to_vc) → ⊨ (P ⋀ Q).to_vc :=
   begin
-    induction H with H₁ f y R S e H₂ σ₂ v ih₁ ih₂,
-
-    show σ ⊨ (calls_to_prop history.empty).instantiated_n, from (
-      have h1: σ ⊨ value.true, from valid_env.true,
-      have (prop.term value.true).erased_n = vc.term value.true, by unfold prop.erased_n,
-      have h2: σ ⊨ (prop.term value.true).erased_n, from this ▸ h1,
-      have calls_n (prop.term value.true) = ∅, from set.eq_empty_of_forall_not_mem (
-        assume c: calltrigger,
-        assume : c ∈ calls_n (prop.term value.true),
-        show «false», from prop.has_call_n.term.inv this
-      ),
-      have (prop.term value.true).instantiated_n = (prop.term value.true).erased_n,
-      from instantiated_n_eq_erased_n_without_calls this,
-      have h3: σ ⊨ (prop.term value.true).instantiated_n, from this.symm ▸ h2, 
-      have calls_to_prop history.empty = value.true, by unfold calls_to_prop,
-      show σ ⊨ (calls_to_prop history.empty).instantiated_n, from this ▸ h3
-    ),
-
-    show σ ⊨ prop.instantiated_n (calls_to_prop (H₁ · call f y R S e H₂ σ₂ v)), from (
-      have h1: σ ⊨ (calls_to_prop H₁).instantiated_n, from ih₁,
-      have h2: σ ⊨ value.true, from valid_env.true,
-      have (prop.call (value.func f y R S e H₂ σ₂) v).erased_n = vc.term value.true, by unfold prop.erased_n,
-      have h3: σ ⊨ (prop.call (value.func f y R S e H₂ σ₂) v).erased_n, from this ▸ h2,
-
-      have quantifiers_n (prop.call (value.func f y R S e H₂ σ₂) v) = ∅, from set.eq_empty_of_forall_not_mem (
-        assume q: callquantifier,
-        assume : q ∈ quantifiers_n (prop.call (value.func f y R S e H₂ σ₂) v),
-        show «false», from prop.has_quantifier_n.call.inv this
-      ),
-      have (prop.call (value.func f y R S e H₂ σ₂) v).instantiated_n
-         = (prop.call (value.func f y R S e H₂ σ₂) v).erased_n,
-      from instantiated_n_eq_erased_n_without_quantifiers this,
-
-      have h4: σ ⊨ (prop.call (value.func f y R S e H₂ σ₂) v).instantiated_n,
-      from this.symm ▸ h3,
-
-      have σ ⊨ ((calls_to_prop H₁).instantiated_n ⋀ (prop.call (value.func f y R S e H₂ σ₂) v).instantiated_n),
-      from valid_env.and h1 h4,
-      have h4: σ ⊨ (calls_to_prop H₁ ⋀ prop.call (value.func f y R S e H₂ σ₂) v).instantiated_n,
-      from valid_env.instantiated_n_and this,
-      have calls_to_prop (H₁ · call f y R S e H₂ σ₂ v)
-        = (calls_to_prop H₁ ⋀ prop.call (value.func f y R S e H₂ σ₂) v),
-      by unfold calls_to_prop,
-      show σ ⊨ (calls_to_prop (H₁ · call f y R S e H₂ σ₂ v)).instantiated_n, from this ▸ h4
-    )
+    assume h1: ⊨ P.to_vc,
+    assume h2: ⊨ Q.to_vc,
+    change ⊨ prop.to_vc (prop.and P Q),
+    unfold prop.to_vc,
+    from valid.and.mp ⟨h1, h2⟩
   end
 
-lemma val_of_free_in_env {P: prop} {σ: env} {x: var}: (⊢ σ : P) → x ∈ FV P → ∃v, σ x = some v :=
-  assume env_verified: ⊢ σ: P,
+lemma valid_env.to_vc_and {P Q: prop} {σ: env}: (σ ⊨ P.to_vc) → (σ ⊨ Q.to_vc) → σ ⊨ (P ⋀ Q).to_vc :=
+  begin
+    assume h1: σ ⊨ P.to_vc,
+    assume h2: σ ⊨ Q.to_vc,
+    change σ ⊨ prop.to_vc (prop.and P Q),
+    unfold prop.to_vc,
+    from valid_env.and h1 h2
+  end
+
+lemma valid_env.to_vc_and.elim {P Q: prop} {σ: env}: (σ ⊨ (P ⋀ Q).to_vc) → ((σ ⊨ P.to_vc) ∧ (σ ⊨ Q.to_vc)) :=
+  begin
+    assume h1: σ ⊨ (P ⋀ Q).to_vc,
+    have h2: σ ⊨ (prop.and P Q).to_vc, from h1,
+    unfold prop.to_vc at h2,
+    from valid_env.and.elim h2
+  end
+
+lemma val_of_free_in_env {P: prop} {σ: env} {x: var}: (⊩ σ : P) → x ∈ FV P → ∃v, σ x = some v :=
+  assume env_verified: ⊩ σ: P,
   assume x_free_in_P: x ∈ FV P,
   have x ∈ σ, from contains_of_free env_verified x_free_in_P,
   show ∃v, σ x = some v, from env.contains_apply_equiv.right.mpr this
 
-lemma val_of_free_in_hist_env {R: spec} {H: history} {σ: env} {P: prop} {x: var}:
-                              (⊢ σ : P) → FV R.to_prop ⊆ FV P → x ∈ FV (R.to_prop ⋀ ↑H ⋀ P) → ∃v, σ x = some v :=
-  assume σ_verified: ⊢ σ : P,
+lemma val_of_free_in_pre_env {R: spec} {σ: env} {P: prop} {x: var}:
+                              (⊩ σ : P) → FV R.to_prop ⊆ FV P → x ∈ FV (R.to_prop ⋀ P) → ∃v, σ x = some v :=
+  assume σ_verified: ⊩ σ : P,
   assume fv_R: FV R.to_prop ⊆ FV P,
-  assume x_free_in_R_H_P: x ∈ FV (R.to_prop ⋀ ↑H ⋀ P),
-  have FV (R.to_prop ⋀ ↑H ⋀ P) = FV ((R.to_prop ⋀ ↑H) ⋀ P), from free_in_prop.and_assoc,
-  have x ∈ FV ((R.to_prop ⋀ ↑H) ⋀ P), from this ▸ x_free_in_R_H_P,
-  have free_in_prop x (R.to_prop ⋀ ↑H) ∨ free_in_prop x P, from free_in_prop.and.inv this,
+  assume x_free_in_R_P: x ∈ FV (R.to_prop ⋀ P),
+  have free_in_prop x R.to_prop ∨ free_in_prop x P, from free_in_prop.and.inv x_free_in_R_P,
   have x ∈ FV P, from or.elim this.symm id (
-    assume : free_in_prop x (R.to_prop ⋀ ↑H),
-    or.elim (free_in_prop.and.inv this) (
-      assume : free_in_prop x R.to_prop,
-      show x ∈ FV P, from set.mem_of_mem_of_subset this fv_R
-    ) (
-      assume : free_in_prop x H,
-      show free_in_prop x P, from absurd this (call_history_closed H x)
-    )
+    assume : free_in_prop x R.to_prop,
+    show x ∈ FV P, from set.mem_of_mem_of_subset this fv_R
   ),
   show ∃v, σ x = some v, from val_of_free_in_env σ_verified this
 
+lemma to_vc_implies {P Q: prop}: (prop.implies P Q).to_vc = vc.implies P.to_vc Q.to_vc :=
+  begin
+    unfold prop.implies,
+    unfold vc.implies,
+    unfold prop.to_vc,
+    congr
+  end
+
+lemma valid.to_vc_implies {P Q: prop}: (⊨ (prop.implies P Q).to_vc) → ⊨ vc.implies P.to_vc Q.to_vc :=
+  begin
+    have h1: ((prop.implies P Q).to_vc = vc.implies P.to_vc Q.to_vc), from to_vc_implies,
+    rw[h1],
+    from id
+  end
+
+lemma valid_env.to_vc_implies {P Q: prop} {σ: env}: (σ ⊨ (prop.implies P Q).to_vc) → σ ⊨ vc.implies P.to_vc Q.to_vc :=
+  begin
+    have h1: ((prop.implies P Q).to_vc = vc.implies P.to_vc Q.to_vc), from to_vc_implies,
+    rw[h1],
+    from id
+  end
+
 lemma simple_equality_valid {σ: env} {x: var} {v: value}:
-  x ∉ σ → (σ[x↦v]) ⊨ (prop.term (x ≡ v)).erased_n :=
+  x ∉ σ → (σ[x↦v]) ⊨ (prop.term (x ≡ v)).to_vc :=
   assume x_not_free_in_σ: x ∉ σ,
   have σ.apply x = none, from env.contains_apply_equiv.left.mpr x_not_free_in_σ,
   have h1: term.subst_env σ x = x, from term.subst_env.var.left.mp this,
@@ -429,98 +419,72 @@ lemma simple_equality_valid {σ: env} {x: var} {v: value}:
   have h6: vc.term (term.subst_env (σ[x↦v]) (x ≡ v)) = vc.term (v ≡ v), by simp[h5],
   have vc.subst_env (σ[x↦v]) (x ≡ v) = vc.term (term.subst_env (σ[x↦v]) (x ≡ v)), from vc.subst_env.term,
   have h7: vc.subst_env (σ[x↦v]) (vc.term (x ≡ v)) = vc.term (v ≡ v), from eq.trans this h6,
-  have prop.erased_n (prop.term (x ≡ v)) = vc.term (x ≡ v), by unfold prop.erased_n,
-  have h8: vc.subst_env (σ[x↦v]) (prop.term (x ≡ v)).erased_n = vc.term (v ≡ v), from this.symm ▸ h7,
+  have prop.to_vc (prop.term (x ≡ v)) = vc.term (x ≡ v), by unfold prop.to_vc,
+  have h8: vc.subst_env (σ[x↦v]) (prop.term (x ≡ v)).to_vc = vc.term (v ≡ v), from this.symm ▸ h7,
   have ⊨ vc.term (v ≡ v), from valid.refl,
-  show (σ[x↦v]) ⊨ prop.erased_n (x ≡ v), from h8.symm ▸ this
+  show (σ[x↦v]) ⊨ prop.to_vc (x ≡ v), from h8.symm ▸ this
 
 lemma simple_equality_env_valid {P: prop} {σ: env} {x: var} {v: value}:
-                                   (⊢ σ: P) → x ∉ σ → (σ ⊨ P.instantiated_n) → ((σ[x↦v]) ⊨ P.instantiated_n)
-                                                             ∧ ((σ[x↦v]) ⊨ (prop.term (x ≡ v)).instantiated_n) :=
-  assume σ_verified: ⊢ σ: P,
+                                     (⊩ σ: P) → x ∉ σ → (σ ⊨ P.to_vc) → (σ[x↦v]) ⊨ (P ⋀ x ≡ v).to_vc :=
+  assume σ_verified: ⊩ σ: P,
   assume x_not_free_in_σ: x ∉ σ,
-  assume ih: σ ⊨ P.instantiated_n,
+  assume ih: σ ⊨ P.to_vc,
   have σ.apply x = none, from env.contains_apply_equiv.left.mpr x_not_free_in_σ,
-  have h1: ⊨ vc.subst_env σ P.instantiated_n, from ih,
-  have x_not_in_P: x ∉ FV (vc.subst_env σ P.instantiated_n), from (
-    assume : x ∈ FV (vc.subst_env σ P.instantiated_n),
-    have x ∈ FV P.instantiated_n, from free_in_vc.subst_env this,
-    have x ∈ FV P, from free_of_instantiated_n_free this,
+  have h1: ⊨ vc.subst_env σ P.to_vc, from ih,
+  have x_not_in_P: x ∉ FV (vc.subst_env σ P.to_vc), from (
+    assume : x ∈ FV (vc.subst_env σ P.to_vc),
+    have x ∈ FV P.to_vc, from free_in_vc.subst_env this,
+    have x ∈ FV P, from set.mem_of_mem_of_subset this free_in_prop_of_free_in_to_vc,
     have ∃v, σ x = some v, from val_of_free_in_env σ_verified this,
     have x ∈ σ, from env.contains_apply_equiv.right.mp this,
     show «false», from x_not_free_in_σ this
   ),
-  have vc.subst x v (vc.subst_env σ P.instantiated_n) = vc.subst_env σ P.instantiated_n,
+  have vc.subst x v (vc.subst_env σ P.to_vc) = vc.subst_env σ P.to_vc,
   from unchanged_of_subst_nonfree_vc x_not_in_P,
-  have h2: ⊨ vc.subst x v (vc.subst_env σ P.instantiated_n),
-  from @eq.subst vc (λa, ⊨ a) (vc.subst_env σ P.instantiated_n)
-          (vc.subst x v (vc.subst_env σ P.instantiated_n)) this.symm h1,
-  have vc.subst x v (vc.subst_env σ P.instantiated_n)
-      = vc.subst_env (σ[x↦v]) P.instantiated_n, by unfold vc.subst_env, 
-  have h3: ⊨ vc.subst_env (σ[x↦v]) P.instantiated_n, from this ▸ h2,
-  have h4: (σ[x↦v]) ⊨ (prop.term (x ≡ v)).erased_n,
+  have h2: ⊨ vc.subst x v (vc.subst_env σ P.to_vc),
+  from @eq.subst vc (λa, ⊨ a) (vc.subst_env σ P.to_vc)
+          (vc.subst x v (vc.subst_env σ P.to_vc)) this.symm h1,
+  have vc.subst x v (vc.subst_env σ P.to_vc)
+      = vc.subst_env (σ[x↦v]) P.to_vc, by unfold vc.subst_env, 
+  have h3: ⊨ vc.subst_env (σ[x↦v]) P.to_vc, from this ▸ h2,
+  have h4: (σ[x↦v]) ⊨ (prop.term (x ≡ v)).to_vc,
   from simple_equality_valid x_not_free_in_σ,
+  have h5: (σ[x↦v]) ⊨ (P.to_vc ⋀ (prop.term (x ≡ v)).to_vc),
+  from valid_env.and h3 h4,
+  have (P.to_vc ⋀ (prop.term (x ≡ v)).to_vc) = prop.to_vc (prop.and P (prop.term (x ≡ v))),
+  by unfold prop.to_vc,
+  have (σ[x↦v]) ⊨ prop.to_vc (prop.and P (prop.term (x ≡ v))), from this ▸ h5,
+  show (σ[x↦v]) ⊨ (P ⋀ x ≡ v).to_vc, from this
 
-  have calls_n (prop.term (x ≡ v)) = ∅, from set.eq_empty_of_forall_not_mem (
-    assume c: calltrigger,
-    assume : c ∈ calls_n (prop.term (x ≡ v)),
-    show «false», from prop.has_call_n.term.inv this
-  ),
-  have (prop.term (x ≡ v)).instantiated_n = (prop.term (x ≡ v)).erased_n,
-  from instantiated_n_eq_erased_n_without_calls this,
-  have (σ[x↦v]) ⊨ (prop.term (x ≡ v)).instantiated_n, from this.symm ▸ h4,
-  ⟨h3, this⟩
-
-lemma simple_equality_env_inst_valid {P: prop} {σ: env} {x: var} {v: value}:
-                                   (⊢ σ: P) → x ∉ σ → (σ ⊨ P.instantiated_n) → (σ[x↦v]) ⊨ (P ⋀ x ≡ v).instantiated_n :=
-  assume σ_verified: ⊢ σ: P,
-  assume x_not_free_in_σ: x ∉ σ,
-  assume ih: σ ⊨ P.instantiated_n,
-  have ((σ[x↦v]) ⊨ P.instantiated_n) ∧ ((σ[x↦v]) ⊨ (prop.term (x ≡ v)).instantiated_n),
-  from simple_equality_env_valid σ_verified x_not_free_in_σ ih,
-  have (σ[x↦v]) ⊨ (P.instantiated_n ⋀ (prop.term (x ≡ v)).instantiated_n),
-  from valid_env.and this.left this.right,
-  show (σ[x↦v]) ⊨ prop.instantiated_n (P ⋀ (x ≡ v)), from valid_env.instantiated_n_and this
-
-lemma env_translation_instantiated_n_valid {P: prop} {σ: env}: (⊢ σ: P) → σ ⊨ P.instantiated_n :=
-  assume env_verified: (⊢ σ : P),
+lemma env_translation_valid {P: prop} {σ: env}: (⊩ σ: P) → σ ⊨ P.to_vc :=
+  assume env_verified: (⊩ σ : P),
   begin
     induction env_verified,
-    case env.vcgen.empty {
-      show env.empty ⊨ prop.instantiated_n (value.true), from (
-        have h: prop.erased_n (prop.term ↑value.true) = vc.term ↑value.true, by unfold prop.erased_n,
-        have env.empty ⊨ value.true, from valid.tru,
-        have h2: env.empty ⊨ prop.erased_n (value.true), from h ▸ this,
-
-        have calls_n (prop.term value.true) = ∅, from set.eq_empty_of_forall_not_mem (
-          assume c: calltrigger,
-          assume : c ∈ calls_n (prop.term value.true),
-          show «false», from prop.has_call_n.term.inv this
-        ),
-        have (prop.term value.true).instantiated_n = (prop.term value.true).erased_n,
-        from instantiated_n_eq_erased_n_without_calls this,
-        
-        show env.empty ⊨ prop.instantiated_n (value.true), from this.symm ▸ h2
-      )
+    case env.dvcgen.empty {
+      unfold vc.subst_env,
+      change ⊨ prop.to_vc (prop.term value.true),
+      unfold prop.to_vc,
+      from valid.tru
     },
-    case env.vcgen.tru σ' x' Q x_not_free_in_σ' σ'_verified ih {
-      show (σ'[x'↦value.true]) ⊨ prop.instantiated_n (Q ⋀ (x' ≡ value.true)),
-      from simple_equality_env_inst_valid σ'_verified x_not_free_in_σ' ih
+    case env.dvcgen.tru σ' x' Q x_not_free_in_σ' σ'_verified ih {
+      from simple_equality_env_valid σ'_verified x_not_free_in_σ' ih
     },
-    case env.vcgen.fls σ' x' Q x_not_free_in_σ' σ'_verified ih {
-      show (σ'[x'↦value.false]) ⊨ prop.instantiated_n (Q ⋀ (x' ≡ value.false)),
-      from simple_equality_env_inst_valid σ'_verified x_not_free_in_σ' ih
+    case env.dvcgen.fls σ' x' Q x_not_free_in_σ' σ'_verified ih {
+      from simple_equality_env_valid σ'_verified x_not_free_in_σ' ih
     },
-    case env.vcgen.num n σ' x' Q x_not_free_in_σ' σ'_verified ih {
-      show (σ'[x'↦value.num n]) ⊨ prop.instantiated_n (Q ⋀ (x' ≡ value.num n)),
-      from simple_equality_env_inst_valid σ'_verified x_not_free_in_σ' ih
+    case env.dvcgen.num n σ' x' Q x_not_free_in_σ' σ'_verified ih {
+      from simple_equality_env_valid σ'_verified x_not_free_in_σ' ih
     },
-    case env.vcgen.func σ₁ σ₂ f g gx R S e H Q₁ Q₂ Q₃
+    case env.dvcgen.func σ₁ σ₂ f g gx R S e Q₁ Q₂ Q₃
       f_not_free_in_σ₁ g_not_free_in_σ₂ gx_not_free_in_σ₂ g_neq_gx σ₁_verified σ₂_verified gx_free_in_R R_fv S_fv func_verified
       S_valid ih₁ ih₂ { from (
-      let vf := value.func g gx R S e H σ₂ in
-      have h1: ((σ₁[f↦vf]) ⊨ Q₁.instantiated_n) ∧ ((σ₁[f↦vf]) ⊨ (prop.term (f ≡ vf)).instantiated_n),
+      let vf := value.func g gx R S e σ₂ in
+      have h1: ((σ₁[f↦vf]) ⊨ (Q₁ ⋀ f ≡ vf).to_vc),
       from simple_equality_env_valid σ₁_verified f_not_free_in_σ₁ ih₁,
+      have h1a: (σ₁[f↦vf]) ⊨ Q₁.to_vc,
+      from (valid_env.to_vc_and.elim h1).left,
+      have h1b: (σ₁[f↦vf]) ⊨ (prop.term (f ≡ vf)).to_vc,
+      from (valid_env.to_vc_and.elim h1).right,
 
       have g_subst: term.subst_env (σ₂[g↦vf]) g = vf, from (
         have h1: term.subst g vf g = vf, from term.subst.var.same,
@@ -531,7 +495,7 @@ lemma env_translation_instantiated_n_valid {P: prop} {σ: env}: (⊢ σ: P) → 
         show term.subst_env (σ₂[g↦vf]) g = vf, from eq.trans this h2
       ),
 
-      have h2: ⊨ prop.instantiated_n (prop.subst_env (σ₂[g↦vf]) (term.unop unop.isFunc g)), from (
+      have h2: ⊨ prop.to_vc (prop.subst_env (σ₂[g↦vf]) (term.unop unop.isFunc g)), from (
         have unop.apply unop.isFunc vf = value.true, by unfold unop.apply,
         have ⊨ (value.true ≡ term.unop unop.isFunc vf), from valid.unop.mp this,
         have ⊨ term.unop unop.isFunc vf, from valid.eq.true.mpr this,
@@ -539,45 +503,31 @@ lemma env_translation_instantiated_n_valid {P: prop} {σ: env}: (⊢ σ: P) → 
         have term.subst_env (σ₂[g↦vf]) (term.unop unop.isFunc g) = term.unop unop.isFunc (term.subst_env (σ₂[g↦vf]) g),
         from term.subst_env.unop,
         have h4: ⊨ vc.term (term.subst_env (σ₂[g↦vf]) (term.unop unop.isFunc g)), from this.symm ▸ h3,
-        have prop.erased_n (prop.term (term.subst_env (σ₂[g↦vf]) (term.unop unop.isFunc g)))
+        have prop.to_vc (prop.term (term.subst_env (σ₂[g↦vf]) (term.unop unop.isFunc g)))
            = vc.term (term.subst_env (σ₂[g↦vf]) (term.unop unop.isFunc g)),
-        by unfold prop.erased_n,
-        have h5: ⊨ prop.erased_n (prop.term (term.subst_env (σ₂[g↦vf]) (term.unop unop.isFunc g))), from this.symm ▸ h4,
+        by unfold prop.to_vc,
+        have h5: ⊨ prop.to_vc (prop.term (term.subst_env (σ₂[g↦vf]) (term.unop unop.isFunc g))), from this.symm ▸ h4,
         have prop.subst_env (σ₂[g↦vf]) (prop.term (term.unop unop.isFunc g))
            = prop.term (term.subst_env (σ₂[g↦vf]) (term.unop unop.isFunc g)), from prop.subst_env.term,
-        have h6: ⊨ prop.erased_n (prop.subst_env (σ₂[g↦vf]) (term.unop unop.isFunc g)), from this.symm ▸ h5,
-
-        have calls_n (prop.subst_env (σ₂[g↦vf]) (term.unop unop.isFunc g)) = ∅, from set.eq_empty_of_forall_not_mem (
-          assume c: calltrigger,
-          assume : c ∈ calls_n (prop.subst_env (σ₂[g↦vf]) (term.unop unop.isFunc g)),
-          have ∃c', c' ∈ calls_n (term.unop unop.isFunc g), from prop.has_call_of_subst_env_has_call.right c this,
-          let ⟨c', h7⟩ := this in
-          show «false», from prop.has_call_n.term.inv h7
-        ),
-        have (prop.subst_env (σ₂[g↦vf]) (term.unop unop.isFunc g)).instantiated_n
-           = (prop.subst_env (σ₂[g↦vf]) (term.unop unop.isFunc g)).erased_n,
-        from instantiated_n_eq_erased_n_without_calls this,
-
-        show ⊨ prop.instantiated_n (prop.subst_env (σ₂[g↦vf]) (term.unop unop.isFunc g)),
-        from this.symm ▸ h6
+        show ⊨ prop.to_vc (prop.subst_env (σ₂[g↦vf]) (term.unop unop.isFunc g)), from this.symm ▸ h5
       ),
 
       let forallp := prop.implies R.to_prop (prop.pre g gx)
                   ⋀ prop.implies (prop.post g gx) (Q₃ (term.app g gx) ⋀ S.to_prop) in
       let pfunc: prop := prop.subst_env (σ₂[g↦vf]) (prop.func g gx R (Q₃ (term.app g gx) ⋀ S)) in
 
-      have h4: ∀v, ⊨ vc.subst gx v (prop.subst_env (σ₂[g↦vf]) forallp).instantiated_n, from (
+      have h4: ∀v, ⊨ vc.subst gx v (prop.subst_env (σ₂[g↦vf]) forallp).to_vc, from (
         assume v: value,
 
-        have h5: ⊨ (prop.subst_env (σ₂[g↦vf][gx↦v]) (prop.implies R.to_prop (prop.pre g gx))).instantiated_n, from (
+        have h5: ⊨ (prop.subst_env (σ₂[g↦vf][gx↦v]) (prop.implies R.to_prop (prop.pre g gx))).to_vc, from (
 
           have h51: (σ₂[g↦vf][gx↦v]).dom = σ₂.dom ∪ {g, gx}, from env.dom.two_elems,
           have σ₂.dom = FV Q₂, from free_iff_contains σ₂_verified,
           have h52: (σ₂[g↦vf][gx↦v]).dom = FV Q₂ ∪ {g, gx}, from this ▸ h51,
           have FV R.to_prop ⊆ (σ₂[g↦vf][gx↦v]).dom, from h52.symm ▸ R_fv,
           have closed (prop.subst_env (σ₂[g↦vf][gx↦v]) R.to_prop), from prop.closed_of_closed_subst this,
-          have h53: closed (prop.subst_env (σ₂[g↦vf][gx↦v]) R.to_prop).instantiated_p,
-          from instantiated_p_closed_of_closed this,
+          have h53: closed (prop.subst_env (σ₂[g↦vf][gx↦v]) R.to_prop).to_vc,
+          from to_vc_closed_of_closed this,
 
           have FV (prop.pre g gx) ⊆ FV Q₂ ∪ {g, gx}, from (
             assume x: var,
@@ -596,16 +546,17 @@ lemma env_translation_instantiated_n_valid {P: prop} {σ: env}: (⊢ σ: P) → 
           ),
           have FV (prop.pre g gx) ⊆ (σ₂[g↦vf][gx↦v]).dom, from h52.symm ▸ this,
           have closed (prop.subst_env (σ₂[g↦vf][gx↦v]) (prop.pre g gx)), from prop.closed_of_closed_subst this,
-          have h54: closed (prop.subst_env (σ₂[g↦vf][gx↦v]) (prop.pre g gx)).instantiated_n,
-          from instantiated_n_closed_of_closed this,
+          have h54: closed (prop.subst_env (σ₂[g↦vf][gx↦v]) (prop.pre g gx)).to_vc,
+          from to_vc_closed_of_closed this,
 
-          have h6: ⊨ vc.implies (prop.subst_env (σ₂[g↦vf][gx↦v]) R.to_prop).instantiated_p
-                                (prop.subst_env (σ₂[g↦vf][gx↦v]) (prop.pre g gx)).instantiated_n,
-          from valid.implies.mp h53 h54 (
-            assume h8: ⊨ (prop.subst_env (σ₂[g↦vf][gx↦v]) R.to_prop).instantiated_p,
-            have vc.subst_env (σ₂[g↦vf][gx↦v]) R.to_prop.instantiated_p
-                = (prop.subst_env (σ₂[g↦vf][gx↦v]) R.to_prop).instantiated_p, from instantiated_p_distrib_subst_env,
-            have ⊨ vc.subst_env (σ₂[g↦vf][gx↦v]) R.to_prop.instantiated_p, from this.symm ▸ h8,
+          have h6: ⊨ vc.implies (prop.subst_env (σ₂[g↦vf][gx↦v]) R.to_prop).to_vc
+                                (prop.subst_env (σ₂[g↦vf][gx↦v]) (prop.pre g gx)).to_vc,
+          from valid.implies.mp (
+            assume h8: ⊨ (prop.subst_env (σ₂[g↦vf][gx↦v]) R.to_prop).to_vc,
+            have vc.subst_env (σ₂[g↦vf][gx↦v]) R.to_prop.to_vc
+                = (prop.subst_env (σ₂[g↦vf][gx↦v]) R.to_prop).to_vc,
+            from subst_env_distrib_to_vc,
+            have ⊨ vc.subst_env (σ₂[g↦vf][gx↦v]) R.to_prop.to_vc, from this.symm ▸ h8,
             have h9: ⊨ vc.pre vf v, from valid.pre.mp this,
             have term.subst gx v gx = v, from term.subst.var.same,
             have h10: ⊨ vc.pre vf (term.subst gx v gx), from this.symm ▸ h9,
@@ -628,44 +579,29 @@ lemma env_translation_instantiated_n_valid {P: prop} {σ: env}: (⊢ σ: P) → 
             by unfold term.subst_env,
             have h14: ⊨ vc.pre (term.subst_env (σ₂[g↦vf][gx↦v]) g) (term.subst_env (σ₂[g↦vf][gx↦v]) gx),
             from this.symm ▸ h13,
-            have prop.erased_n (prop.pre (term.subst_env (σ₂[g↦vf][gx↦v]) g) (term.subst_env (σ₂[g↦vf][gx↦v]) gx))
+            have prop.to_vc (prop.pre (term.subst_env (σ₂[g↦vf][gx↦v]) g) (term.subst_env (σ₂[g↦vf][gx↦v]) gx))
                = (vc.pre (term.subst_env (σ₂[g↦vf][gx↦v]) g) (term.subst_env (σ₂[g↦vf][gx↦v]) gx)),
-            by unfold prop.erased_n,
-            have h15: ⊨ (prop.pre (term.subst_env (σ₂[g↦vf][gx↦v]) g) (term.subst_env (σ₂[g↦vf][gx↦v]) gx)).erased_n,
+            by unfold prop.to_vc,
+            have h15: ⊨ (prop.pre (term.subst_env (σ₂[g↦vf][gx↦v]) g) (term.subst_env (σ₂[g↦vf][gx↦v]) gx)).to_vc,
             from this.symm ▸ h14,
             have prop.subst_env (σ₂[g↦vf][gx↦v]) (prop.pre g gx)
                = prop.pre (term.subst_env (σ₂[g↦vf][gx↦v]) g) (term.subst_env (σ₂[g↦vf][gx↦v]) gx),
             from prop.subst_env.pre,
-            have h16: ⊨ (prop.subst_env (σ₂[g↦vf][gx↦v]) (prop.pre g gx)).erased_n, from this.symm ▸ h15,
-
-            have calls_n (prop.subst_env (σ₂[g↦vf][gx↦v]) (prop.pre g gx)) = ∅,
-            from set.eq_empty_of_forall_not_mem (
-              assume c: calltrigger,
-              assume : c ∈ calls_n (prop.subst_env (σ₂[g↦vf][gx↦v]) (prop.pre g gx)),
-              have ∃c', c' ∈ calls_n (prop.pre g gx), from prop.has_call_of_subst_env_has_call.right c this,
-              let ⟨c', h17⟩ := this in
-              show «false», from prop.has_call_n.pre.inv h17
-            ),
-            have (prop.subst_env (σ₂[g↦vf][gx↦v]) (prop.pre g gx)).instantiated_n
-              = (prop.subst_env (σ₂[g↦vf][gx↦v]) (prop.pre g gx)).erased_n,
-            from instantiated_n_eq_erased_n_without_calls this,
-
-            show ⊨ (prop.subst_env (σ₂[g↦vf][gx↦v]) (prop.pre g gx)).instantiated_n,
-            from this.symm ▸ h16
+            show ⊨ (prop.subst_env (σ₂[g↦vf][gx↦v]) (prop.pre g gx)).to_vc, from this.symm ▸ h15
           ),
           have h8: ⊨ (prop.implies (prop.subst_env (σ₂[g↦vf][gx↦v]) R.to_prop)
-                                   (prop.subst_env (σ₂[g↦vf][gx↦v]) (prop.pre g gx))).instantiated_n,
-          from valid.instantiated_n_implies h6,
+                                   (prop.subst_env (σ₂[g↦vf][gx↦v]) (prop.pre g gx))).to_vc,
+          from valid.to_vc_implies h6,
           have prop.subst_env (σ₂[g↦vf][gx↦v]) (prop.implies R.to_prop (prop.pre g gx))
              = prop.implies (prop.subst_env (σ₂[g↦vf][gx↦v]) R.to_prop)
                             (prop.subst_env (σ₂[g↦vf][gx↦v]) (prop.pre g gx)),
           from prop.subst_env.implies,
-          show ⊨ (prop.subst_env (σ₂[g↦vf][gx↦v]) (prop.implies R.to_prop (prop.pre g gx))).instantiated_n,
+          show ⊨ (prop.subst_env (σ₂[g↦vf][gx↦v]) (prop.implies R.to_prop (prop.pre g gx))).to_vc,
           from this.symm ▸ h8
         ),
 
         have h6: ⊨ (prop.subst_env (σ₂[g↦vf][gx↦v]) (prop.implies (prop.post g gx)
-                                                     (Q₃ (term.app g gx) ⋀ S.to_prop))).instantiated_n, from (
+                                                     (Q₃ (term.app g gx) ⋀ S.to_prop))).to_vc, from (
 
           have h61: (σ₂[g↦vf][gx↦v]).dom = σ₂.dom ∪ {g, gx}, from env.dom.two_elems,
           have σ₂.dom = FV Q₂, from free_iff_contains σ₂_verified,
@@ -676,7 +612,7 @@ lemma env_translation_instantiated_n_valid {P: prop} {σ: env}: (⊢ σ: P) → 
             assume : x ∈ FV (Q₃ (term.app g gx) ⋀ S.to_prop),
             or.elim (free_in_prop.and.inv this) (
               assume : x ∈ FV (Q₃ (term.app g gx)),
-              have x ∈ FV (term.app g gx) ∨ x ∈ FV (↑H ⋀ Q₂ ⋀ spec.func ↑g gx R S ⋀ R),
+              have x ∈ FV (term.app g gx) ∨ x ∈ FV (Q₂ ⋀ spec.func ↑g gx R S ⋀ R),
               from exp.post_free func_verified (term.app g gx) this,
               or.elim this (
                 assume : x ∈ FV (term.app g gx),
@@ -692,95 +628,80 @@ lemma env_translation_instantiated_n_valid {P: prop} {σ: env}: (⊢ σ: P) → 
                   show x ∈ FV Q₂ ∪ {g, gx}, from set.mem_union_right (FV Q₂) this
                 )
               ) (
-                assume : x ∈ FV (↑H ⋀ Q₂ ⋀ spec.func ↑g gx R S ⋀ R),
+                assume : x ∈ FV (Q₂ ⋀ spec.func ↑g gx R S ⋀ R),
                 or.elim (free_in_prop.and.inv this) (
-                  assume : free_in_prop x H,
-                  show x ∈ FV Q₂ ∪ {g, gx}, from absurd this (call_history_closed H x)
+                  assume : x ∈ FV Q₂,
+                  show x ∈ FV Q₂ ∪ {g, gx}, from set.mem_union_left {g, gx} this
                 ) (
-                  assume : x ∈ FV (Q₂ ⋀ spec.func ↑g gx R S ⋀ R),
+                  assume : free_in_prop x (spec.func ↑g gx R S ⋀ R),
+                  have free_in_prop x (spec.func ↑g gx R S ⋀ R), from this,
                   or.elim (free_in_prop.and.inv this) (
-                    assume : x ∈ FV Q₂,
-                    show x ∈ FV Q₂ ∪ {g, gx}, from set.mem_union_left {g, gx} this
-                  ) (
-                    assume : free_in_prop x (spec.func ↑g gx R S ⋀ R),
-                    have free_in_prop x (spec.func ↑g gx R S ⋀ R), from this,
+                    assume : free_in_prop x (spec.func ↑g gx R S),
+                    have h63: free_in_prop x (spec.func ↑g gx R S).to_prop, from this,
+                    have spec.to_prop (spec.func ↑g gx R S) = (prop.func ↑g gx R.to_prop S.to_prop),
+                    by unfold spec.to_prop,
+                    have h64: free_in_prop x (prop.func ↑g gx R S), from this ▸ h63,
+                    let forallp := prop.implies R.to_prop (prop.pre g gx)
+                                ⋀ prop.implies (prop.post g gx) S.to_prop in
+                    have prop.func g gx R.to_prop S.to_prop
+                      = (term.unop unop.isFunc g ⋀ prop.forallc gx forallp),
+                    by unfold prop.func,
+                    have free_in_prop x (term.unop unop.isFunc g ⋀ prop.forallc gx forallp),
+                    from this ▸ h64,
                     or.elim (free_in_prop.and.inv this) (
-                      assume : free_in_prop x (spec.func ↑g gx R S),
-                      have h63: free_in_prop x (spec.func ↑g gx R S).to_prop, from this,
-                      have spec.to_prop (spec.func ↑g gx R S) = (prop.func ↑g gx R.to_prop S.to_prop),
-                      by unfold spec.to_prop,
-                      have h64: free_in_prop x (prop.func ↑g gx R S), from this ▸ h63,
-                      let forallp := prop.implies R.to_prop (prop.pre g gx)
-                                  ⋀ prop.implies (prop.post g gx) S.to_prop in
-                      have prop.func g gx R.to_prop S.to_prop
-                        = (term.unop unop.isFunc g ⋀ prop.forallc gx g forallp),
-                      by unfold prop.func,
-                      have free_in_prop x (term.unop unop.isFunc g ⋀ prop.forallc gx g forallp),
-                      from this ▸ h64,
+                      assume : free_in_prop x (term.unop unop.isFunc g),
+                      have free_in_term x (term.unop unop.isFunc g), from free_in_prop.term.inv this,
+                      have free_in_term x g, from free_in_term.unop.inv this,
+                      have x = g, from free_in_term.var.inv this,
+                      have x ∈ {g, gx}, from set.two_elems_mem.inv (or.inl this),
+                      show x ∈ FV Q₂ ∪ {g, gx}, from set.mem_union_right (FV Q₂) this
+                    ) (
+                      assume : free_in_prop x (prop.forallc gx forallp),
+                      have x_neq_gx: x ≠ gx, from (free_in_prop.forallc.inv this).left,
+                      have free_in_prop x forallp, from (free_in_prop.forallc.inv this).right,
                       or.elim (free_in_prop.and.inv this) (
-                        assume : free_in_prop x (term.unop unop.isFunc g),
-                        have free_in_term x (term.unop unop.isFunc g), from free_in_prop.term.inv this,
-                        have free_in_term x g, from free_in_term.unop.inv this,
-                        have x = g, from free_in_term.var.inv this,
-                        have x ∈ {g, gx}, from set.two_elems_mem.inv (or.inl this),
-                        show x ∈ FV Q₂ ∪ {g, gx}, from set.mem_union_right (FV Q₂) this
-                      ) (
-                        assume : free_in_prop x (prop.forallc gx g forallp),
-                        have x_neq_gx: x ≠ gx, from (free_in_prop.forallc.inv this).left,
-                        have free_in_term x g ∨ free_in_prop x forallp,
-                        from (free_in_prop.forallc.inv this).right,
-                        or.elim this (
-                          assume : free_in_term x g,
-                          have x = g, from free_in_term.var.inv this,
-                          have x ∈ {g, gx}, from set.two_elems_mem.inv (or.inl this),
-                          show x ∈ FV Q₂ ∪ {g, gx}, from set.mem_union_right (FV Q₂) this
+                        assume : free_in_prop x (prop.implies R.to_prop (prop.pre g gx)),
+                        or.elim (free_in_prop.implies.inv this) (
+                          assume : free_in_prop x R.to_prop,
+                          show x ∈ FV Q₂ ∪ {g, gx}, from R_fv this
                         ) (
-                          assume : free_in_prop x forallp,
-                          or.elim (free_in_prop.and.inv this) (
-                            assume : free_in_prop x (prop.implies R.to_prop (prop.pre g gx)),
-                            or.elim (free_in_prop.implies.inv this) (
-                              assume : free_in_prop x R.to_prop,
-                              show x ∈ FV Q₂ ∪ {g, gx}, from R_fv this
-                            ) (
-                              assume : x ∈ FV (prop.pre g gx),
-                              or.elim (free_in_prop.pre.inv this) (
-                                assume : free_in_term x g,
-                                have x = g, from free_in_term.var.inv this,
-                                have x ∈ {g, gx}, from set.two_elems_mem.inv (or.inl this),
-                                show x ∈ FV Q₂ ∪ {g, gx}, from set.mem_union_right (FV Q₂) this
-                              ) (
-                                assume : free_in_term x gx,
-                                have x = gx, from free_in_term.var.inv this,
-                                have x ∈ {g, gx}, from set.two_elems_mem.inv (or.inr this),
-                                show x ∈ FV Q₂ ∪ {g, gx}, from set.mem_union_right (FV Q₂) this
-                              )
-                            )
+                          assume : x ∈ FV (prop.pre g gx),
+                          or.elim (free_in_prop.pre.inv this) (
+                            assume : free_in_term x g,
+                            have x = g, from free_in_term.var.inv this,
+                            have x ∈ {g, gx}, from set.two_elems_mem.inv (or.inl this),
+                            show x ∈ FV Q₂ ∪ {g, gx}, from set.mem_union_right (FV Q₂) this
                           ) (
-                            assume : free_in_prop x (prop.implies (prop.post g gx) S.to_prop),
-                            or.elim (free_in_prop.implies.inv this) (
-                              assume : x ∈ FV (prop.post g gx),
-                              or.elim (free_in_prop.post.inv this) (
-                                assume : free_in_term x g,
-                                have x = g, from free_in_term.var.inv this,
-                                have x ∈ {g, gx}, from set.two_elems_mem.inv (or.inl this),
-                                show x ∈ FV Q₂ ∪ {g, gx}, from set.mem_union_right (FV Q₂) this
-                              ) (
-                                assume : free_in_term x gx,
-                                have x = gx, from free_in_term.var.inv this,
-                                have x ∈ {g, gx}, from set.two_elems_mem.inv (or.inr this),
-                                show x ∈ FV Q₂ ∪ {g, gx}, from set.mem_union_right (FV Q₂) this
-                              )
-                            ) (
-                              assume : free_in_prop x S.to_prop,
-                              show x ∈ FV Q₂ ∪ {g, gx}, from S_fv this
-                            )
+                            assume : free_in_term x gx,
+                            have x = gx, from free_in_term.var.inv this,
+                            have x ∈ {g, gx}, from set.two_elems_mem.inv (or.inr this),
+                            show x ∈ FV Q₂ ∪ {g, gx}, from set.mem_union_right (FV Q₂) this
                           )
                         )
+                      ) (
+                        assume : free_in_prop x (prop.implies (prop.post g gx) S.to_prop),
+                        or.elim (free_in_prop.implies.inv this) (
+                          assume : x ∈ FV (prop.post g gx),
+                          or.elim (free_in_prop.post.inv this) (
+                            assume : free_in_term x g,
+                            have x = g, from free_in_term.var.inv this,
+                            have x ∈ {g, gx}, from set.two_elems_mem.inv (or.inl this),
+                            show x ∈ FV Q₂ ∪ {g, gx}, from set.mem_union_right (FV Q₂) this
+                          ) (
+                            assume : free_in_term x gx,
+                            have x = gx, from free_in_term.var.inv this,
+                            have x ∈ {g, gx}, from set.two_elems_mem.inv (or.inr this),
+                            show x ∈ FV Q₂ ∪ {g, gx}, from set.mem_union_right (FV Q₂) this
+                          )
+                        ) (
+                          assume : free_in_prop x S.to_prop,
+                          show x ∈ FV Q₂ ∪ {g, gx}, from S_fv this
+                        )
                       )
-                    ) (
-                      assume : free_in_prop x R,
-                      show x ∈ FV Q₂ ∪ {g, gx}, from R_fv this
                     )
+                  ) (
+                    assume : free_in_prop x R,
+                    show x ∈ FV Q₂ ∪ {g, gx}, from R_fv this
                   )
                 )
               )
@@ -793,8 +714,8 @@ lemma env_translation_instantiated_n_valid {P: prop} {σ: env}: (⊢ σ: P) → 
           have FV (Q₃ (term.app g gx) ⋀ S.to_prop) ⊆ (σ₂[g↦vf][gx↦v]).dom, from h62.symm ▸ this,
           have closed (prop.subst_env (σ₂[g↦vf][gx↦v]) (Q₃ (term.app g gx) ⋀ S.to_prop)),
           from prop.closed_of_closed_subst this,
-          have h63: closed (prop.subst_env (σ₂[g↦vf][gx↦v]) (Q₃ (term.app g gx) ⋀ S.to_prop)).instantiated_n,
-          from instantiated_n_closed_of_closed this,
+          have h63: closed (prop.subst_env (σ₂[g↦vf][gx↦v]) (Q₃ (term.app g gx) ⋀ S.to_prop)).to_vc,
+          from to_vc_closed_of_closed this,
 
           have FV (prop.post g gx) ⊆ FV Q₂ ∪ {g, gx}, from (
             assume x: var,
@@ -813,41 +734,23 @@ lemma env_translation_instantiated_n_valid {P: prop} {σ: env}: (⊢ σ: P) → 
           ),
           have FV (prop.post g gx) ⊆ (σ₂[g↦vf][gx↦v]).dom, from h62.symm ▸ this,
           have closed (prop.subst_env (σ₂[g↦vf][gx↦v]) (prop.post g gx)), from prop.closed_of_closed_subst this,
-          have h64: closed (prop.subst_env (σ₂[g↦vf][gx↦v]) (prop.post g gx)).instantiated_p,
-          from instantiated_p_closed_of_closed this,
+          have h64: closed (prop.subst_env (σ₂[g↦vf][gx↦v]) (prop.post g gx)).to_vc,
+          from to_vc_closed_of_closed this,
 
-          have h7: ⊨ vc.implies (prop.subst_env (σ₂[g↦vf][gx↦v]) (prop.post g gx)).instantiated_p
-                                (prop.subst_env (σ₂[g↦vf][gx↦v]) (Q₃ (term.app g gx) ⋀ S.to_prop)).instantiated_n,
-          from valid.implies.mp h64 h63 (
-            assume h8: ⊨ (prop.subst_env (σ₂[g↦vf][gx↦v]) (prop.post g gx)).instantiated_p,
+          have h7: ⊨ vc.implies (prop.subst_env (σ₂[g↦vf][gx↦v]) (prop.post g gx)).to_vc
+                                (prop.subst_env (σ₂[g↦vf][gx↦v]) (Q₃ (term.app g gx) ⋀ S.to_prop)).to_vc,
+          from valid.implies.mp (
+            assume h8: ⊨ (prop.subst_env (σ₂[g↦vf][gx↦v]) (prop.post g gx)).to_vc,
             have prop.subst_env (σ₂[g↦vf][gx↦v]) (prop.post g gx)
                = prop.post (term.subst_env (σ₂[g↦vf][gx↦v]) g) (term.subst_env (σ₂[g↦vf][gx↦v]) gx),
             from prop.subst_env.post,
-            have h81: ⊨ (prop.post (term.subst_env (σ₂[g↦vf][gx↦v]) g) (term.subst_env (σ₂[g↦vf][gx↦v]) gx))
-                          .instantiated_p,
+            have h9: ⊨ (prop.post (term.subst_env (σ₂[g↦vf][gx↦v]) g)
+                                  (term.subst_env (σ₂[g↦vf][gx↦v]) gx)).to_vc,
             from this ▸ h8,
 
-            have calls_p (prop.post (term.subst_env (σ₂[g↦vf][gx↦v]) g)
-                                    (term.subst_env (σ₂[g↦vf][gx↦v]) gx)) = ∅,
-            from set.eq_empty_of_forall_not_mem (
-              assume c: calltrigger,
-              assume : c ∈ calls_p (prop.post (term.subst_env (σ₂[g↦vf][gx↦v]) g)
-                                   (term.subst_env (σ₂[g↦vf][gx↦v]) gx)),
-              show «false», from prop.has_call_p.post.inv this
-            ),
-            have (prop.post (term.subst_env (σ₂[g↦vf][gx↦v]) g)
-                            (term.subst_env (σ₂[g↦vf][gx↦v]) gx)).instantiated_p
-              = (prop.post (term.subst_env (σ₂[g↦vf][gx↦v]) g)
-                           (term.subst_env (σ₂[g↦vf][gx↦v]) gx)).erased_p,
-            from instantiated_p_eq_erased_p_without_calls this,
-
-            have h9: ⊨ (prop.post (term.subst_env (σ₂[g↦vf][gx↦v]) g)
-                                  (term.subst_env (σ₂[g↦vf][gx↦v]) gx)).erased_p,
-            from this ▸ h81,
-
-            have (prop.post (term.subst_env (σ₂[g↦vf][gx↦v]) g) (term.subst_env (σ₂[g↦vf][gx↦v]) gx)).erased_n
+            have (prop.post (term.subst_env (σ₂[g↦vf][gx↦v]) g) (term.subst_env (σ₂[g↦vf][gx↦v]) gx)).to_vc
                 = vc.post (term.subst_env (σ₂[g↦vf][gx↦v]) g) (term.subst_env (σ₂[g↦vf][gx↦v]) gx),
-            by unfold prop.erased_n,
+            by unfold prop.to_vc,
             have h10: ⊨ vc.post (term.subst_env (σ₂[g↦vf][gx↦v]) g) (term.subst_env (σ₂[g↦vf][gx↦v]) gx),
             from this ▸ h9,
             have term.subst_env (σ₂[g↦vf][gx↦v]) g = term.subst gx v (term.subst_env (σ₂[g↦vf]) g),
@@ -867,143 +770,123 @@ lemma env_translation_instantiated_n_valid {P: prop} {σ: env}: (⊢ σ: P) → 
             have h14: ⊨ vc.post vf (term.subst gx v gx), from this ▸ h13,
             have term.subst gx v gx = v, from term.subst.var.same,
             have ⊨ vc.post vf v, from this ▸ h14,
-            have (σ₂[g↦vf][gx↦v] ⊨ (Q₃ (term.app g gx)).instantiated_n ⋀ S.to_prop.instantiated_n),
+            have (σ₂[g↦vf][gx↦v] ⊨ (Q₃ (term.app g gx)).to_vc ⋀ S.to_prop.to_vc),
             from valid.post.mpr σ₂_verified func_verified this,
-            have h15: (σ₂[g↦vf][gx↦v] ⊨ (Q₃ (term.app g gx) ⋀ S.to_prop).instantiated_n),
-            from valid_env.instantiated_n_and this,
-            have vc.subst_env (σ₂[g↦vf][gx↦v]) (Q₃ (term.app g gx) ⋀ S.to_prop).instantiated_n
-              = (prop.subst_env (σ₂[g↦vf][gx↦v]) (Q₃ (term.app g gx) ⋀ S.to_prop)).instantiated_n,
-            from instantiated_n_distrib_subst_env,
-            show ⊨ (prop.subst_env (σ₂[g↦vf][gx↦v]) (Q₃ (term.app g gx) ⋀ S.to_prop)).instantiated_n,
+            have h15: (σ₂[g↦vf][gx↦v] ⊨ (Q₃ (term.app g gx) ⋀ S.to_prop).to_vc),
+            from valid_env.to_vc_and (valid_env.and.elim this).left (valid_env.and.elim this).right,
+            have vc.subst_env (σ₂[g↦vf][gx↦v]) (Q₃ (term.app g gx) ⋀ S.to_prop).to_vc
+              = (prop.subst_env (σ₂[g↦vf][gx↦v]) (Q₃ (term.app g gx) ⋀ S.to_prop)).to_vc,
+            from subst_env_distrib_to_vc,
+            show ⊨ (prop.subst_env (σ₂[g↦vf][gx↦v]) (Q₃ (term.app g gx) ⋀ S.to_prop)).to_vc,
             from this ▸ h15
           ),
           have h8: ⊨ (prop.implies (prop.subst_env (σ₂[g↦vf][gx↦v]) (prop.post g gx))
-                                   (prop.subst_env (σ₂[g↦vf][gx↦v]) (Q₃ (term.app g gx) ⋀ S.to_prop))).instantiated_n,
-          from valid.instantiated_n_implies h7,
+                                   (prop.subst_env (σ₂[g↦vf][gx↦v]) (Q₃ (term.app g gx) ⋀ S.to_prop))).to_vc,
+          from valid.to_vc_implies h7,
           have prop.subst_env (σ₂[g↦vf][gx↦v]) (prop.implies (prop.post g gx) (Q₃ (term.app g gx) ⋀ S.to_prop))
              = prop.implies (prop.subst_env (σ₂[g↦vf][gx↦v]) (prop.post g gx))
                             (prop.subst_env (σ₂[g↦vf][gx↦v]) (Q₃ (term.app g gx) ⋀ S.to_prop)),
           from prop.subst_env.implies,
           show ⊨ (prop.subst_env (σ₂[g↦vf][gx↦v]) (prop.implies (prop.post g gx)
-                                                      (Q₃ (term.app g gx) ⋀ S.to_prop))).instantiated_n,
+                                                      (Q₃ (term.app g gx) ⋀ S.to_prop))).to_vc,
           from this.symm ▸ h8
         ),
 
-        have ⊨ ((prop.subst_env (σ₂[g↦vf][gx↦v]) (prop.implies R.to_prop (prop.pre g gx))).instantiated_n ⋀
-                (prop.subst_env (σ₂[g↦vf][gx↦v]) (prop.implies (prop.post g gx)
-                                                                (Q₃ (term.app g gx) ⋀ S.to_prop))).instantiated_n),
-        from valid.and.mp ⟨h5, h6⟩,
         have h7: ⊨ (prop.subst_env (σ₂[g↦vf][gx↦v]) (prop.implies R.to_prop (prop.pre g gx)) ⋀
                     prop.subst_env (σ₂[g↦vf][gx↦v]) (prop.implies (prop.post g gx)
-                                                                   (Q₃ (term.app g gx) ⋀ S.to_prop))).instantiated_n,
-        from valid.instantiated_n_and this,
+                                                                   (Q₃ (term.app g gx) ⋀ S.to_prop))).to_vc,
+        from valid.to_vc_and h5 h6,
         have prop.subst_env (σ₂[g↦vf][gx↦v]) forallp
            = (prop.subst_env (σ₂[g↦vf][gx↦v]) (prop.implies R.to_prop (prop.pre g gx)) ⋀
              prop.subst_env (σ₂[g↦vf][gx↦v]) (prop.implies (prop.post g gx) (Q₃ (term.app g gx) ⋀ S.to_prop))),
         from prop.subst_env.and,
-        have h8: ⊨ (prop.subst_env (σ₂[g↦vf][gx↦v]) forallp).instantiated_n, from this.symm ▸ h7,
+        have h8: ⊨ (prop.subst_env (σ₂[g↦vf][gx↦v]) forallp).to_vc, from this.symm ▸ h7,
         have prop.subst_env (σ₂[g↦vf][gx↦v]) forallp = prop.subst gx v (prop.subst_env (σ₂[g↦vf]) forallp),
         by unfold prop.subst_env,
-        have h9: ⊨ (prop.subst gx v (prop.subst_env (σ₂[g↦vf]) forallp)).instantiated_n, from this ▸ h8,
-        have vc.subst gx v (prop.subst_env (σ₂[g↦vf]) forallp).instantiated_n
-           = (prop.subst gx v (prop.subst_env (σ₂[g↦vf]) forallp)).instantiated_n, from instantiated_n_distrib_subst,
-        show ⊨ vc.subst gx v (prop.subst_env (σ₂[g↦vf]) forallp).instantiated_n, from this.symm ▸ h9
+        have h9: ⊨ (prop.subst gx v (prop.subst_env (σ₂[g↦vf]) forallp)).to_vc, from this ▸ h8,
+        have vc.subst gx v (prop.subst_env (σ₂[g↦vf]) forallp).to_vc
+           = (prop.subst gx v (prop.subst_env (σ₂[g↦vf]) forallp)).to_vc,
+        from subst_distrib_to_vc,
+        show ⊨ vc.subst gx v (prop.subst_env (σ₂[g↦vf]) forallp).to_vc, from this.symm ▸ h9
       ),
 
-      have h5: ⊨ prop.instantiated_n (prop.subst_env (σ₂[g↦vf]) (prop.forallc gx g forallp)), from (
-        have h6: ⊨ vc.univ gx (prop.subst_env (σ₂[g↦vf]) forallp).instantiated_n, from valid.univ.mp h4,
-        have prop.instantiated_n (prop.forallc gx (term.subst_env (σ₂[g↦vf]) g) (prop.subst_env (σ₂[g↦vf]) forallp))
-           = vc.univ gx (prop.subst_env (σ₂[g↦vf]) forallp).instantiated_n, from instantiated_n.forallc,
-        have h7: ⊨ prop.instantiated_n (prop.forallc gx (term.subst_env (σ₂[g↦vf]) g) (prop.subst_env (σ₂[g↦vf]) forallp)), from this.symm ▸ h6,
+      have h5: ⊨ prop.to_vc (prop.subst_env (σ₂[g↦vf]) (prop.forallc gx forallp)), from (
+        have h6: ⊨ vc.univ gx (prop.subst_env (σ₂[g↦vf]) forallp).to_vc, from valid.univ.mp h4,
+        have prop.to_vc (prop.forallc gx (prop.subst_env (σ₂[g↦vf]) forallp))
+           = vc.univ gx (prop.subst_env (σ₂[g↦vf]) forallp).to_vc,
+        by unfold prop.to_vc,
+        have h7: ⊨ prop.to_vc (prop.forallc gx (prop.subst_env (σ₂[g↦vf]) forallp)), from this.symm ▸ h6,
         have ¬(gx = g ∨ gx ∈ σ₂), from not_or_distrib.mpr ⟨g_neq_gx.symm, gx_not_free_in_σ₂⟩,
         have gx ∉ (σ₂[g↦vf]), from (mt env.contains.inv) this,
-        have (prop.subst_env (σ₂[g↦vf]) (prop.forallc gx g forallp)
-            = prop.forallc gx (term.subst_env (σ₂[g↦vf]) g) (prop.subst_env (σ₂[g↦vf]) forallp)),
+        have (prop.subst_env (σ₂[g↦vf]) (prop.forallc gx forallp)
+            = prop.forallc gx (prop.subst_env (σ₂[g↦vf]) forallp)),
         from prop.subst_env.forallc_not_in this,
-        show ⊨ prop.instantiated_n (prop.subst_env (σ₂[g↦vf]) (prop.forallc gx g forallp)), from this.symm ▸ h7
+        show ⊨ prop.to_vc (prop.subst_env (σ₂[g↦vf]) (prop.forallc gx forallp)), from this.symm ▸ h7
       ),
 
-      have ⊨ (prop.instantiated_n (prop.subst_env (σ₂[g↦vf]) (term.unop unop.isFunc g)) ⋀
-                  prop.instantiated_n (prop.subst_env (σ₂[g↦vf]) (prop.forallc gx g forallp))),
-      from valid.and.mp ⟨h2, h5⟩,
-      have h7: ⊨ prop.instantiated_n (prop.subst_env (σ₂[g↦vf]) (term.unop unop.isFunc g) ⋀
-                                    prop.subst_env (σ₂[g↦vf]) (prop.forallc gx g forallp)),
-      from valid.instantiated_n_and this,
-      have prop.subst_env (σ₂[g↦vf]) (term.unop unop.isFunc g ⋀ prop.forallc gx g forallp)
-         = (prop.subst_env (σ₂[g↦vf]) (term.unop unop.isFunc g) ⋀ prop.subst_env (σ₂[g↦vf]) (prop.forallc gx g forallp)),
+      have h7: ⊨ prop.to_vc (prop.subst_env (σ₂[g↦vf]) (term.unop unop.isFunc g) ⋀
+                             prop.subst_env (σ₂[g↦vf]) (prop.forallc gx forallp)),
+      from valid.to_vc_and h2 h5,
+      have prop.subst_env (σ₂[g↦vf]) (term.unop unop.isFunc g ⋀ prop.forallc gx forallp)
+         = (prop.subst_env (σ₂[g↦vf]) (term.unop unop.isFunc g) ⋀ prop.subst_env (σ₂[g↦vf]) (prop.forallc gx forallp)),
       from prop.subst_env.and,
-      have h8: ⊨ prop.instantiated_n (prop.subst_env (σ₂[g↦vf]) (term.unop unop.isFunc g ⋀ prop.forallc gx g forallp)),
+      have h8: ⊨ prop.to_vc (prop.subst_env (σ₂[g↦vf]) (term.unop unop.isFunc g ⋀ prop.forallc gx forallp)),
       from this.symm ▸ h7,
       have prop.func g gx R.to_prop (Q₃ (term.app g gx) ⋀ S.to_prop)
-         = (term.unop unop.isFunc g ⋀ prop.forallc gx g forallp),
+         = (term.unop unop.isFunc g ⋀ prop.forallc gx forallp),
       by unfold prop.func,
-      have ⊨ prop.instantiated_n (prop.subst_env (σ₂[g↦vf]) (prop.func g gx R (Q₃ (term.app g gx) ⋀ S))),
+      have ⊨ prop.to_vc (prop.subst_env (σ₂[g↦vf]) (prop.func g gx R (Q₃ (term.app g gx) ⋀ S))),
       from this.symm ▸ h8,
-      have h9: ⊨ prop.instantiated_n pfunc, from this,
+      have h9: ⊨ prop.to_vc pfunc, from this,
 
       have h10: (∀x, x ∉ FV pfunc), from (
-        have ⊢ (σ₂[g↦vf]) : Q₂
+        have ⊩ (σ₂[g↦vf]) : Q₂
           ⋀ (g ≡ (vf))
           ⋀ prop.subst_env (σ₂[g↦vf]) (prop.func g gx R (Q₃ (term.app g gx) ⋀ S)),
-        from env.vcgen.func g_not_free_in_σ₂ g_not_free_in_σ₂ gx_not_free_in_σ₂ g_neq_gx
+        from env.dvcgen.func g_not_free_in_σ₂ g_not_free_in_σ₂ gx_not_free_in_σ₂ g_neq_gx
              σ₂_verified σ₂_verified gx_free_in_R R_fv S_fv func_verified S_valid,
         prop_func_closed this
       ),
 
-      have h11: (∀x, x ∉ FV pfunc.instantiated_n), from (
+      have h11: (∀x, x ∉ FV pfunc.to_vc), from (
         assume x: var,
-        assume : x ∈ FV pfunc.instantiated_n,
-        have x ∈ FV pfunc, from free_of_instantiated_n_free this,
+        assume : x ∈ FV pfunc.to_vc,
+        have x ∈ FV pfunc, from set.mem_of_mem_of_subset this free_in_prop_of_free_in_to_vc,
         show «false», from (h10 x) this
       ),
 
-      have vc.subst_env (σ₁[f↦vf]) pfunc.instantiated_n = pfunc.instantiated_n,
+      have vc.subst_env (σ₁[f↦vf]) pfunc.to_vc = pfunc.to_vc,
       from unchanged_of_subst_env_nonfree_vc h11 (σ₁[f↦vf]),
-      have (σ₁[f↦vf]) ⊨ pfunc.instantiated_n, from this.symm ▸ h9,
+      have (σ₁[f↦vf]) ⊨ pfunc.to_vc, from this.symm ▸ h9,
 
-      have (σ₁[f↦vf]) ⊨ ((prop.term (f ≡ vf)).instantiated_n ⋀ prop.instantiated_n pfunc), from valid_env.and h1.right this,
-      have (σ₁[f↦vf]) ⊨ ((prop.term (f ≡ vf)) ⋀ pfunc).instantiated_n, from valid_env.instantiated_n_and this,
-      have (σ₁[f↦vf]) ⊨ Q₁.instantiated_n ⋀ ((prop.term (f ≡ vf)) ⋀ pfunc).instantiated_n, from valid_env.and h1.left this,
-      show (σ₁[f↦vf]) ⊨ (Q₁ ⋀ (f ≡ vf) ⋀ pfunc).instantiated_n,
-      from valid_env.instantiated_n_and this
+      have (σ₁[f↦vf]) ⊨ ((prop.term (f ≡ vf)) ⋀ pfunc).to_vc,
+      from valid_env.to_vc_and h1b this,
+      show (σ₁[f↦vf]) ⊨ (Q₁ ⋀ (f ≡ vf) ⋀ pfunc).to_vc,
+      from valid_env.to_vc_and h1a this
     )}
   end
 
-lemma env_translation_valid {R: spec} {H: history} {P: prop} {σ: env}:
-  (⊢ σ: P) → (σ ⊨ R.to_prop.instantiated_n) → σ ⊨ (↑R ⋀ ↑H ⋀ P).instantiated_n :=
-  assume env_verified: (⊢ σ : P),
-  assume R_valid: (σ ⊨ R.to_prop.instantiated_n),
-  have h1: σ ⊨ prop.instantiated_n ↑H, from history_valid σ,
-  have h2: σ ⊨ P.instantiated_n, from env_translation_instantiated_n_valid env_verified,
-  have σ ⊨ (prop.instantiated_n ↑H ⋀ P.instantiated_n), from valid_env.and h1 h2,
-  have σ ⊨ (↑H ⋀ P).instantiated_n, from valid_env.instantiated_n_and this,
-  have σ ⊨ R.to_prop.instantiated_n ⋀ (↑H ⋀ P).instantiated_n, from valid_env.and R_valid this,
-  show σ ⊨ (↑R ⋀ ↑H ⋀ P).instantiated_n, from valid_env.instantiated_n_and this
-
-lemma consequent_of_H_P {R: spec} {H: history} {σ: env} {P Q: prop}:
-      (⊢ σ: P) → closed_subst σ R.to_prop → (σ ⊨ R.to_prop.instantiated_n) →
-     closed_subst σ Q → ⟪prop.implies (R ⋀ ↑H ⋀ P) Q⟫ → σ ⊨ Q.instantiated_p :=
-  assume env_verified: (⊢ σ : P),
+lemma consequent_of_pre_P {R: spec} {σ: env} {P Q: prop}:
+      (⊩ σ: P) → closed_subst σ R.to_prop → (σ ⊨ R.to_prop.to_vc) →
+     closed_subst σ Q → ⦃ prop.implies (R ⋀ P) Q ⦄ → σ ⊨ Q.to_vc :=
+  assume env_verified: (⊩ σ : P),
   assume R_closed: closed_subst σ R.to_prop,
-  assume R_valid: (σ ⊨ R.to_prop.instantiated_n),
+  assume R_valid: (σ ⊨ R.to_prop.to_vc),
   assume Q_closed: closed_subst σ Q,
-  assume : ⟪prop.implies (R ⋀ ↑H ⋀ P) Q⟫,
-  have impl: σ ⊨ (prop.implies (↑R ⋀ ↑H ⋀ P) Q).instantiated_n, from this σ,
-  have closed (calls_to_prop H), from call_history_closed H,
-  have h1: closed_subst σ (calls_to_prop H), from prop.closed_any_subst_of_closed this,
+  assume vc_valid: ⦃ prop.implies (R ⋀ P) Q ⦄,
+
   have closed_subst σ P, from env_translation_closed_subst env_verified,
-  have closed_subst σ (↑H ⋀ P), from prop.closed_subst.and h1 this,
-  have closed_subst σ (↑R ⋀ ↑H ⋀ P), from prop.closed_subst.and R_closed this,
-  have closed_subst σ (prop.implies (↑R ⋀ ↑H ⋀ P) Q), from prop.closed_subst.implies this Q_closed,
-  have closed_subst σ (prop.implies (↑R ⋀ ↑H ⋀ P) Q).instantiated_p, from instantiated_p_closed_subst_of_closed this,
-  have σ ⊨ (prop.implies (↑R ⋀ ↑H ⋀ P) Q).instantiated_p, from valid_env.instantiated_p_of_instantiated_n this impl,
-  have σ ⊨ ((↑R ⋀ ↑H ⋀ P).not ⋁ Q).instantiated_p, from this,
-  have h2: σ ⊨ ((↑R ⋀ ↑H ⋀ P).not.instantiated_p ⋁ Q.instantiated_p), from valid_env.instantiated_p_or_elim this,
-  have (↑R ⋀ ↑H ⋀ P).not.instantiated_p = (↑R ⋀ ↑H ⋀ P).instantiated_n.not, from not_dist_instantiated_p,
-  have σ ⊨ ((↑R ⋀ ↑H ⋀ P).instantiated_n.not ⋁ Q.instantiated_p), from this ▸ h2,
-  have h3: σ ⊨ vc.implies (↑R ⋀ ↑H ⋀ P).instantiated_n Q.instantiated_p, from this,
-  have σ ⊨ (↑R ⋀ ↑H ⋀ P).instantiated_n, from env_translation_valid env_verified R_valid,
-  show σ ⊨ Q.instantiated_p, from valid_env.mp h3 this
+  have closed_subst σ (↑R ⋀ P), from prop.closed_subst.and R_closed this,
+  have closed_subst σ (prop.implies (↑R ⋀ P) Q), from prop.closed_subst.implies this Q_closed,
+  have impl: σ ⊨ (prop.implies (↑R ⋀ P) Q).to_vc, from vc_valid σ this,
+  have (prop.implies (↑R ⋀ P) Q).to_vc = vc.implies (↑R ⋀ P).to_vc Q.to_vc,
+  by { unfold prop.implies, unfold vc.implies, unfold prop.to_vc, congr },
+  have impl2: σ ⊨ vc.implies (↑R ⋀ P).to_vc Q.to_vc, from this ▸ impl,
+  have σ ⊨ P.to_vc, from env_translation_valid env_verified,
+  have σ ⊨ (↑R ⋀ P).to_vc, from valid_env.to_vc_and R_valid this,
+  show σ ⊨ Q.to_vc, from valid_env.mp impl2 this
+
+/-
 
 lemma env_translation_call_valid {R: spec} {H: history} {P: prop} {σ: env} {f x: var}:
   (⊢ σ: P) → (σ ⊨ R.to_prop.instantiated_n) → σ ⊨ ((↑R ⋀ ↑H ⋀ P) ⋀ prop.call f x).instantiated_n :=
@@ -1035,50 +918,44 @@ lemma env_translation_call_valid {R: spec} {H: history} {P: prop} {σ: env} {f x
   have σ ⊨ (↑R ⋀ ↑H ⋀ P).instantiated_n ⋀ (prop.call f x).instantiated_n, from valid_env.and h3 this,
   show σ ⊨ ((↑R ⋀ ↑H ⋀ P) ⋀ prop.call f x).instantiated_n, from valid_env.instantiated_n_and this
 
-lemma consequent_of_H_P_call {R: spec} {H: history} {σ: env} {P Q: prop} {f x: var}:
-  (⊢ σ: P) → closed_subst σ R.to_prop → (σ ⊨ R.to_prop.instantiated_n) →
-  ⟪prop.implies ((↑R ⋀ ↑H ⋀ P) ⋀ prop.call f x) Q⟫ → f ∈ σ → x ∈ σ → closed_subst σ Q → σ ⊨ Q.instantiated_p :=
-  assume env_verified: (⊢ σ : P),
-  assume R_closed: closed_subst σ R.to_prop,
-  assume R_valid: (σ ⊨ R.to_prop.instantiated_n),
-  assume impl_vc: ⟪prop.implies ((↑R ⋀ ↑H ⋀ P) ⋀ prop.call f x) Q⟫,
-  assume f_in_σ: f ∈ σ,
-  assume x_in_σ: x ∈ σ,
-  assume Q_closed: closed_subst σ Q,
-  have h1: σ ⊨ (prop.implies ((↑R ⋀ ↑H ⋀ P) ⋀ prop.call f x) Q).instantiated_n, from impl_vc σ,
+-/
 
-  have closed (calls_to_prop H), from call_history_closed H,
-  have h2: closed_subst σ (calls_to_prop H), from prop.closed_any_subst_of_closed this,
+lemma consequent_of_pre_P_call {R: spec} {σ: env} {P Q: prop} {x: var}:
+      (⊩ σ: P) → closed_subst σ R.to_prop → (σ ⊨ R.to_prop.to_vc) → x ∈ σ →
+     closed_subst σ Q → ⦃ prop.implies ((R ⋀ P) ⋀ prop.call x) Q ⦄ → σ ⊨ Q.to_vc :=
+  assume env_verified: (⊩ σ : P),
+  assume R_closed: closed_subst σ R.to_prop,
+  assume R_valid: (σ ⊨ R.to_prop.to_vc),
+  assume env_has_x: x ∈ σ,
+  assume Q_closed: closed_subst σ Q,
+  assume vc_valid: ⦃ prop.implies ((R ⋀ P) ⋀ prop.call x) Q ⦄,
+
   have closed_subst σ P, from env_translation_closed_subst env_verified,
-  have closed_subst σ (↑H ⋀ P), from prop.closed_subst.and h2 this,
-  have h10: closed_subst σ (↑R ⋀ ↑H ⋀ P), from prop.closed_subst.and R_closed this,
-  have closed_subst σ (prop.call f x), from (
-    assume z: var,
-    assume : z ∈ FV (prop.call f x),
-    or.elim (free_in_prop.call.inv this) (
-      assume : free_in_term z f,
-      have z = f, from free_in_term.var.inv this,
-      show z ∈ σ, from this.symm ▸ f_in_σ
-    ) (
-      assume : free_in_term z x,
-      have z = x, from free_in_term.var.inv this,
-      show z ∈ σ, from this.symm ▸ x_in_σ
-    )
-  ),
-  have closed_subst σ ((↑R ⋀ ↑H ⋀ P) ⋀ prop.call f x), from prop.closed_subst.and h10 this,
-  have closed_subst σ (prop.implies ((↑R ⋀ ↑H ⋀ P) ⋀ prop.call f x) Q), from prop.closed_subst.implies this Q_closed,
-  have closed_subst σ (prop.implies ((↑R ⋀ ↑H ⋀ P) ⋀ prop.call f x) Q).instantiated_p,
-  from instantiated_p_closed_subst_of_closed this,
-  have σ ⊨ (prop.implies ((↑R ⋀ ↑H ⋀ P) ⋀ prop.call f x) Q).instantiated_p,
-  from valid_env.instantiated_p_of_instantiated_n this h1,
-  have σ ⊨ (((↑R ⋀ ↑H ⋀ P) ⋀ prop.call f x).not ⋁ Q).instantiated_p, from this,
-  have h2: σ ⊨ (((↑R ⋀ ↑H ⋀ P) ⋀ prop.call f x).not.instantiated_p ⋁ Q.instantiated_p), from valid_env.instantiated_p_or_elim this,
-  have ((↑R ⋀ ↑H ⋀ P) ⋀ prop.call f x).not.instantiated_p = ((↑R ⋀ ↑H ⋀ P) ⋀ prop.call f x).instantiated_n.not,
-  from not_dist_instantiated_p,
-  have σ ⊨ (((↑R ⋀ ↑H ⋀ P) ⋀ prop.call f x).instantiated_n.not ⋁ Q.instantiated_p), from this ▸ h2,
-  have h3: σ ⊨ vc.implies ((↑R ⋀ ↑H ⋀ P) ⋀ prop.call f x).instantiated_n Q.instantiated_p, from this,
-  have σ ⊨ ((↑R ⋀ ↑H ⋀ P) ⋀ prop.call f x).instantiated_n, from env_translation_call_valid env_verified R_valid,
-  show σ ⊨ Q.instantiated_p, from valid_env.mp h3 this
+  have h1: closed_subst σ (↑R ⋀ P), from prop.closed_subst.and R_closed this,
+  have closed_subst σ (prop.call x), by begin
+    assume y: var,
+    assume h1,
+    have h2, from free_in_prop.call.inv h1,
+    have h3: (y = x), from free_in_term.var.inv h2,
+    rw[←h3] at env_has_x,
+    from env_has_x
+  end,
+  have closed_subst σ ((↑R ⋀ P) ⋀ prop.call x), from prop.closed_subst.and h1 this,
+  have closed_subst σ (prop.implies ((↑R ⋀ P) ⋀ prop.call x) Q),
+  from prop.closed_subst.implies this Q_closed,
+  have impl: σ ⊨ (prop.implies ((↑R ⋀ P) ⋀ prop.call x) Q).to_vc, from vc_valid σ this,
+  have (prop.implies (↑R ⋀ P) Q).to_vc = vc.implies (↑R ⋀ P).to_vc Q.to_vc,
+  by { unfold prop.implies, unfold vc.implies, unfold prop.to_vc, congr },
+  have impl2: σ ⊨ vc.implies ((↑R ⋀ P) ⋀ prop.call x).to_vc Q.to_vc, from this ▸ impl,
+  have σ ⊨ P.to_vc, from env_translation_valid env_verified,
+  have h2: σ ⊨ (↑R ⋀ P).to_vc, from valid_env.to_vc_and R_valid this,
+  have h3: σ ⊨ value.true, from valid_env.true,
+  have prop.to_vc (prop.call x) = value.true, by { unfold prop.to_vc, congr },
+  have σ ⊨ (prop.call x).to_vc, from this.symm ▸ h3,
+  have σ ⊨ ((↑R ⋀ P) ⋀ prop.call x).to_vc, from valid_env.to_vc_and h2 this,
+  show σ ⊨ Q.to_vc, from valid_env.mp impl2 this
+
+/-
 
 lemma dominates_p_equiv_subst {σ₁ σ₂: env} {P: prop}:
   (∀y, y ∈ σ₁ → (σ₁ y = σ₂ y)) → dominates_p σ₂ (prop.subst_env σ₁ P) P :=
